progress

HOL_To_IMP/Refinements/HOL_TCN_To_IMP_Temp.thy
@@ -1,14 +1,17 @@
 theory HOL_TCN_To_IMP_Temp
-  imports HOL_To_IMP_Primitives "IMP.HOL_TCN_To_IMP"
+  imports HOL_To_IMP_Primitives "IMP.HOL_TCN_To_IMP" (* HOL_Nat_To_IMP.Compile_HOL_Nat_To_IMP *)
+(* TODO: rearrange import of stuff from Compile *)
 begin
 
-(*
-  (* assumes inf: "\<exists>zh v. (f,reg) \<turnstile> (t,vs_b,vs_arg) \<Rightarrow>\<^bsup>zh\<^esup> v" *)
+method repeat methods m = (m; repeat \<open>m\<close>)?
 
-(* definition "interp_time1 reg g vs_arg_g = T_f_from_reg reg g vs_arg_g" *)
-(* definition "interp_time reg = sum_map (\<lambda>(g, vs_arg_g). interp_time1 reg g vs_arg_g)" *)
-  (* assumes "f_imp = to_imp_tc_1 f_args ctxt r0 f" *)
-  (* assumes "set (special_regs f_args ctxt r t) \<subseteq> set stale" *)
+(*
+  (* assumes inf: "\<exists>zh v. (f,frgt) \<turnstile> (t,vs_b,vs_arg) \<Rightarrow>\<^bsup>zh\<^esup> v" *)
+
+(* definition "interp_time1 frgt g vs_arg_g = T_f_from_reg frgt g vs_arg_g" *)
+(* definition "interp_time frgt = sum_map (\<lambda>(g, vs_arg_g). interp_time1 frgt g vs_arg_g)" *)
+  (* assumes "f_imp = to_imp_tc_1 f_args crgt r0 f" *)
+  (* assumes "set (special_regs f_args crgt r t) \<subseteq> set stale" *)
 
 abbreviation "lookups names (s :: state) \<equiv> map s names"
 
@@ -17,57 +20,581 @@ definition "is_call_in t f = (f \<in> set (calls t))"
 lemma lookups_eq_on: assumes "s = t on set xs" shows "lookups xs s = lookups xs t"
   using assms by (simp add: eq_on_def)
 
-abbreviation "lookup_args ctxt g \<equiv> lookups (args_from_ctxt ctxt g)"
+abbreviation "lookup_args crgt g \<equiv> lookups (args_from_crgt crgt g)"
 
-definition "tinterp_time reg ctxt =
+definition "tinterp_time frgt crgt =
   sum_map
     (\<lambda>(g, vs_arg_g).
-      HOL_Nat_To_IMP.least_constant_IMP (com_from_ctxt ctxt g) (T_f_from_reg reg g o lookup_args ctxt g)
-      * interp_time1 reg g vs_arg_g)"
+      HOL_Nat_To_IMP.least_constant_IMP (com_from_crgt crgt g) (T_f_from_reg frgt g o lookup_args crgt g)
+      * interp_time1 frgt g vs_arg_g)"
 
 *)
 
 abbreviation "lookups names (s :: state) \<equiv> map s names"
-abbreviation "lookup_args ctxt g \<equiv> lookups (args_from_ctxt ctxt g)"
+abbreviation "lookup_args crgt g \<equiv> lookups (args_from_crgt crgt g)"
 
 (* definition "is_call_in t f = (f \<in> set (calls t))" *)
 
-definition "well_formed_comp f_args ctxt bs stale t \<longleftrightarrow>
+(* the term is tail-recursive, "special" registers are marked stale,
+   and the argument list of f and of any called functions is distinct *)
+definition "compiler_args_invar f_args crgt bs stale t \<longleftrightarrow>
   HOL_TCN_Timing.invar t
-  \<and> set (reserved_regs f_args ctxt bs t) \<subseteq> set stale
+  \<and> set (reserved_regs f_args crgt bs t) \<subseteq> set stale
   \<and> distinct f_args
-  \<and> (\<forall>g \<in> set (calls t). distinct (args_from_ctxt ctxt g))"
+  \<and> (\<forall>(g,_) \<in> set (calls t). distinct (args_from_crgt crgt g))
+  \<and> (\<forall>(g,ts) \<in> set (calls t). length ts = length (args_from_crgt crgt g))"
 
-definition "well_encoded_comp f_args bs vs_arg vs_b s \<longleftrightarrow> lookups f_args s = vs_arg \<and> lookups bs s = vs_b"
+(* the "state" of the HOL-TCN execution (args, bounds) is related
+   to the state of the IMP-TC execution *)
+definition "relate_exec_state f_args bs vs_arg vs_b s \<longleftrightarrow>
+  lookups f_args s = vs_arg \<and> lookups bs s = vs_b"
 
-definition "called_correctness ctxt reg t \<longleftrightarrow> (\<forall>g \<in> set (calls t).
+definition "called_correctness crgt frgt fs \<longleftrightarrow> (\<forall>f \<in> fs.
     HOL_Nat_To_IMP.terminates_with_res_time_order_IMP
-      (com_from_ctxt ctxt g) (ret_from_ctxt ctxt g)
-      (f_from_reg reg g o lookup_args ctxt g) (T_f_from_reg reg g o lookup_args ctxt g))" (* can we replace f with existential ? *)
+      (com_from_crgt crgt f) (ret_from_crgt crgt f)
+      (f_from_frgt frgt f o lookup_args crgt f) (T_f_from_frgt frgt f o lookup_args crgt f))" (* can we replace ...  with existential ? *)
+
+definition "relate_rgt_correctness frgt crgt fs \<longleftrightarrow> (\<forall>f \<in> fs.
+  \<forall>s. terminates_with_res_IMP (com_from_crgt crgt f) s (ret_from_crgt crgt f)
+        (f_from_frgt frgt f (lookup_args crgt f s)))"
+
+
+(* note: lookups xs s = map s xs *)
+lemma map_eq_on_subset_eq: fixes A assumes "set xs \<subseteq> A" "f = g on A" shows "map f xs = map g xs"
+  using assms unfolding eq_on_def by (induction xs) auto
+
+lemma snoc_obtain:
+  assumes "xs \<noteq> []"
+  obtains x xs' where "xs = xs' @ [x]"
+  using assms by (meson rev_exhaust)
+
+lemma snoc_list_induct2 [case_names len Nil snoc]:
+  assumes len: "length xs = length ys"
+  assumes nil: "P [] []"
+  assumes snoc: "\<And>xs x ys y. length xs = length ys \<Longrightarrow> P xs ys \<Longrightarrow> P (xs @ [x]) (ys @ [y])"
+  shows "P xs ys"
+proof-
+  let ?P = "\<lambda>xs ys. P (rev xs) (rev ys)"
+  have "length (rev xs) = length (rev ys)" using len by simp
+  then have "?P (rev xs) (rev ys)"
+  proof (induction rule: list_induct2)
+  qed (simp_all add: nil snoc)
+  then show "P xs ys" by simp
+qed
+
+lemma snoc_list_induct3 [case_names len1 len2 Nil snoc]:
+  assumes len: "length xs = length ys" "length ys = length zs"
+  assumes nil: "P [] [] []"
+  assumes snoc: "\<And>xs x ys y zs z. length xs = length ys \<Longrightarrow> length ys = length zs \<Longrightarrow> P xs ys zs \<Longrightarrow> P (xs @ [x]) (ys @ [y]) (zs @ [z])"
+  shows "P xs ys zs"
+proof-
+  let ?P = "\<lambda>xs ys zs. P (rev xs) (rev ys) (rev zs)"
+  have "length (rev xs) = length (rev ys)" "length (rev ys) = length (rev zs)" using len by simp_all
+  then have "?P (rev xs) (rev ys) (rev zs)"
+  proof (induction rule: list_induct3)
+  qed (simp_all add: nil snoc)
+  then show "P xs ys zs" by simp
+qed
+
+  
+(* 
+lemma snoc_list_induct3 [case_names len1 len2 Nil snoc]:
+  assumes "length ys = length xs"
+  assumes "length zs = length xs"
+  assumes nil: "P [] [] []"
+  assumes cons: "\<And>xs x ys y zs z. length ys = length xs \<Longrightarrow> length zs = length xs \<Longrightarrow> P xs ys zs \<Longrightarrow> P (xs @ [x]) (ys @ [y]) (zs @ [z])"
+  shows "P xs ys zs"
+using assms(1,2) proof (induction "rev xs" arbitrary: xs ys zs)
+  case (Cons a as')
+  then have "xs \<noteq> []" "ys \<noteq> []" "zs \<noteq> []" by auto
+  then obtain x xs' y ys' z zs' where "xs = xs' @ [x]" "ys = ys' @ [y]" "zs = zs' @ [z]" using snoc_obtain by metis
+  then moreover have "length ys' = length xs'" "length zs' = length xs'" using Cons by simp_all
+  ultimately show ?case using Cons cons by simp
+qed (simp add: nil) *)
 
 (*
-lemma ttime_non_tail:
-  fixes c :: tcom
-  assumes "invar c"
-  assumes "f \<turnstile> (c,s1) \<Rightarrow>\<^bsup>z\<^esup> s2"
-  assumes "teval_to_tail s1 c None"
-  shows "ttime_to_tail s1 c z"
-  sorry (* TODO *)
+lemma mapi_ix1:
+  assumes "length ys = length xs"
+  shows "map (\<lambda>i. f ((ys @ zs) ! i) i) [0..<length xs] = map (\<lambda>i. f (ys ! i) i) [0..<length xs]"
+  apply simp apply (subst nth_append) using assms apply simp done
 
-lemma non_tail_tailrec: "non_tail t \<Longrightarrow> tailrec t"
-  by (induction t) auto *)
+lemma mapi_ix2:
+  assumes "length ys = length xs"
+  assumes "zs \<noteq> []"
+  shows "(\<lambda>i. f ((ys @ zs) ! i) i) (length xs) = f (hd zs) (length xs)"
+  apply (subst nth_append) using assms hd_conv_nth by fastforce *)
 
-(* TODO: need assumption relating registry and context *)
+(* lemma nth_append1:
+  assumes "n < length xs"
+  shows "(xs @ ys) ! n = xs ! n"
+  using assms nth_append by metis *)
+
+lemma nth_append_length_eq:
+  assumes "length xs = length ys"
+  shows "(xs @ y # zs) ! (length ys) = y"
+  apply (subst nth_append) using assms by simp
+
+lemma copy_list_sem:
+  assumes "length xs = length ys"
+  assumes "distinct (xs @ ys)" (* technically, this assumption could be weakened *)
+  obtains s' where
+    "f \<turnstile> (t_seqs' (map (\<lambda>i. (ys ! i) ::= A (V (xs ! i))) [0..<length xs]),s) \<Rightarrow>\<^bsup>Suc (2 * length xs)\<^esup> s'"
+    "lookups xs s = lookups ys s'" "s = s' on (- set ys)"
+using assms proof (induction xs ys arbitrary: thesis rule: snoc_list_induct2)
+  case Nil
+  then show ?case using tSkip_tE by auto
+next
+  case (snoc xs x ys y)
+
+  let ?cs = "\<lambda>xs ys. map (\<lambda>i. (ys ! i) ::= A (V (xs ! i)) :: tcom) [0..<length xs]"
+
+  let ?cs1 = "?cs xs ys"
+  let ?c2 = "y ::= A (V x) :: tcom"
+  let ?cs' = "?cs (xs @ [x]) (ys @ [y])"
+
+  have cs': "?cs' = ?cs1 @ [?c2]" by (simp add: snoc nth_append_left nth_append_length_eq)
+
+  from snoc obtain s2 where ih:
+      "f \<turnstile> (t_seqs' ?cs1, s) \<Rightarrow>\<^bsup>Suc (2 * length xs)\<^esup> s2"
+      "lookups xs s = lookups ys s2" "s = s2 on (- set ys)"
+    by auto
+  moreover obtain s3 where step:
+      "f \<turnstile> (?c2, s2) \<Rightarrow>\<^bsup>Suc (Suc 0)\<^esup> s3"
+      "s3 y = s2 x" "s2 = s3 on (- {y})"
+    by fastforce
+  ultimately have "f \<turnstile> (t_seqs' ?cs1;; ?c2, s) \<Rightarrow>\<^bsup>Suc (2 * length (xs @ [x]))\<^esup> s3" by auto
+  then have "f \<turnstile> (t_seqs' (?cs1 @ [?c2]), s) \<Rightarrow>\<^bsup>Suc (2 * length (xs @ [x]))\<^esup> s3" 
+    using t_seqs'_snoc t_seqs'_t_seqs by simp
+  then have 1: "f \<turnstile> (t_seqs' ?cs', s) \<Rightarrow>\<^bsup>Suc (2 * length (xs @ [x]))\<^esup> s3"
+    by (subst cs') assumption
+
+  have 2: "lookups (xs @ [x]) s = lookups (ys @ [y]) s3"
+    using ih step snoc by auto
+
+  have 3: "s = s3 on (- set (ys @ [y]))"
+    using ih step by auto
+
+  from 1 2 3 snoc show ?case by blast
+qed (simp add: assms)
+
+
+
+lemma cc_call_helper:
+  "f \<turnstile> (t_seqs' cs1;; t_seqs' cs2;; c, s) \<Rightarrow>\<^bsup>Suc (Suc z)\<^esup> t \<longleftrightarrow> f \<turnstile> (t_seqs (cs1 @ cs2) c, s) \<Rightarrow>\<^bsup>z\<^esup> t"
+  using tbig_step_t_t_seqs_rewrite by simp
+
+abbreviation "calls_r t \<equiv> set (map fst (calls t))"
+
 lemma compiler_correct_nt:
   assumes "\<not> tails t"
-  assumes "well_formed_comp f_args ctxt bs stale t"
-  assumes "well_encoded_comp f_args bs vs_arg vs_b s"
-  obtains f z s' where
-    "f \<turnstile> (to_imp_tc f_args ctxt bs r stale t,s) \<Rightarrow>\<^bsup>z\<^esup> s'"
-    "s' r = eval_non_tail reg vs_b vs_arg t" (* TODO *)
-    "s = s' on (Set.remove r (set stale))"
-  nitpick
-  sorry
+  assumes "(f,frgt) \<turnstile> (t,vs_b,vs_arg) \<Rightarrow>\<^bsup>z\<^esup> v"
+  assumes "compiler_args_invar f_args crgt bs stale t"
+  assumes "relate_rgt_correctness frgt crgt (calls_r t)"
+  assumes "relate_exec_state f_args bs vs_arg vs_b s"
+  shows "\<exists>z_c s'.
+    f_c \<turnstile> (to_imp_tc f_args crgt bs r stale t,s) \<Rightarrow>\<^bsup>z_c\<^esup> s'
+    \<and> s' r = v
+    \<and> s = s' on set stale - {r}"
+using assms proof (induction t arbitrary: vs_b z v bs stale s r crgt)
+  case (hLet t1 t2)
+
+  let ?r1 = "fresh' stale ''Let.x''"
+
+  have no_tails: "\<not> HOL_TCN_Timing.tails t1" "\<not> HOL_TCN_Timing.tails t2" using hLet by simp_all
+
+  obtain z1 v1 z2 where inv: "z = z1 + z2" "(f, frgt) \<turnstile> (t1, vs_b, vs_arg) \<Rightarrow>\<^bsup>z1\<^esup>  v1" "(f, frgt) \<turnstile> (t2, v1 # vs_b, vs_arg) \<Rightarrow>\<^bsup>z2\<^esup>  v"
+    using hLet_case hLet.prems by blast
+
+  have args_invar: "compiler_args_invar f_args crgt bs stale t1" "compiler_args_invar f_args crgt (?r1 # bs) (?r1 # stale) t2"
+    using hLet unfolding compiler_args_invar_def reserved_regs_def split_beta by auto
+
+  have rel_rgt: "relate_rgt_correctness frgt crgt (calls_r t1)" "relate_rgt_correctness frgt crgt (calls_r t2)"
+    using hLet unfolding relate_rgt_correctness_def by auto
+
+  have rel_state1: "relate_exec_state f_args bs vs_arg vs_b s" using hLet by blast
+
+  obtain z1_c s2 where
+    ih1: "f_c \<turnstile> (to_imp_tc f_args crgt bs ?r1 stale t1, s) \<Rightarrow>\<^bsup>z1_c\<^esup>  s2" "s2 ?r1 = v1" "s = s2 on set stale - {?r1}"
+    using no_tails inv args_invar rel_rgt rel_state1 hLet by metis
+
+  have res_reg_subset: "set f_args \<subseteq> set stale - {?r1}" "set bs \<subseteq> set stale - {?r1}"
+    using hLet.prems(3) fresh_not_in_stale unfolding compiler_args_invar_def reserved_regs_def by simp_all
+
+  have rel_state2: "relate_exec_state f_args (?r1 # bs) vs_arg (v1 # vs_b) s2"
+    using hLet ih1 unfolding relate_exec_state_def apply simp
+    unfolding map_eq_on_subset_eq[OF res_reg_subset(1)] map_eq_on_subset_eq[OF res_reg_subset(2)] by blast
+
+  obtain z2_c s3 where
+    ih2: "f_c \<turnstile> (to_imp_tc f_args crgt (?r1 # bs) r (?r1 # stale) t2, s2) \<Rightarrow>\<^bsup>z2_c\<^esup>  s3" "s3 r = v" "s2 = s3 on set (?r1 # stale) - {r}"
+    using hLet.IH(2)[OF no_tails(2) inv(3) args_invar(2) rel_rgt(2) rel_state2] by blast
+
+  have "s = s2 on set stale - {r}" using ih1 fresh_not_in_stale eq_on_subset by blast
+  moreover have "s2 = s3 on set stale - {r}" using ih2 fresh_not_in_stale by auto
+  ultimately have s3_like_s: "s = s3 on set stale - {r}" by blast
+
+  show ?case
+    apply (simp add: Let_def)
+    apply (repeat \<open>rule exI\<close>; repeat \<open>rule conjI\<close>)
+    apply (rule tbig_step_t.tSeq)
+    using ih1 ih2 s3_like_s by auto
+next
+  case (hLetBound n)
+  show ?case
+  proof (repeat \<open>rule exI\<close>; repeat \<open>rule conjI\<close>)
+    from hLetBound_case hLetBound have "v = vs_b ! n" "n < length vs_b" by auto
+    then have "aval (A (V (bs ! n))) s = v" using hLetBound unfolding relate_exec_state_def by auto
+    then show "f_c \<turnstile> (to_imp_tc f_args crgt bs r stale (hLetBound n), s) \<Rightarrow>\<^bsup>Suc (Suc 0)\<^esup> s(r := v)"
+      by (metis tbig_step_t.tAssign to_imp_tc.simps(3))
+  qed (simp_all add: eq_on_def)
+next
+  case (hArg n)
+  show ?case
+  proof (repeat \<open>rule exI\<close>; repeat \<open>rule conjI\<close>)
+    from hArg_case hArg have "v = vs_arg ! n" "n < length vs_arg" by auto
+    then have "aval (A (V (f_args ! n))) s = v" using hArg unfolding relate_exec_state_def by auto
+    then show "f_c \<turnstile> (to_imp_tc f_args crgt bs r stale (hArg n), s) \<Rightarrow>\<^bsup>Suc (Suc 0)\<^esup> s(r := v)"
+      by (metis tbig_step_t.tAssign to_imp_tc.simps(4))
+  qed (simp_all add: eq_on_def)
+next
+  case (hNumber n)
+  show ?case
+  proof (repeat \<open>rule exI\<close>; repeat \<open>rule conjI\<close>)
+    have "aval (A (N n)) s = v" using hNumber unfolding relate_exec_state_def by auto
+    then show "f_c \<turnstile> (to_imp_tc f_args crgt bs r stale (hNumber n), s) \<Rightarrow>\<^bsup>Suc (Suc 0)\<^esup> s(r := v)"
+      by (metis tbig_step_t.tAssign to_imp_tc.simps(5))
+  qed (simp_all add: eq_on_def)
+next
+  case (hIf t1 t2 t3)
+
+  let ?r1 = "fresh' stale ''If.x''"
+
+  have no_tails: "\<not> HOL_TCN_Timing.tails t1" "\<not> HOL_TCN_Timing.tails t2" "\<not> HOL_TCN_Timing.tails t3" using hIf by simp_all
+
+  have args_invar: "compiler_args_invar f_args crgt bs stale t1" "compiler_args_invar f_args crgt bs stale t2" "compiler_args_invar f_args crgt bs stale t3"
+    using hIf unfolding compiler_args_invar_def reserved_regs_def split_beta by auto
+
+  have rel_rgt: "relate_rgt_correctness frgt crgt (calls_r t1)" "relate_rgt_correctness frgt crgt (calls_r t2)" "relate_rgt_correctness frgt crgt (calls_r t3)"
+    using hIf unfolding relate_rgt_correctness_def by auto
+
+  have rel_state1: "relate_exec_state f_args bs vs_arg vs_b s" using hIf by blast
+
+  have res_reg_subset: "set f_args \<subseteq> set stale - {?r1}" "set bs \<subseteq> set stale - {?r1}"
+    using hIf.prems(3) fresh_not_in_stale unfolding compiler_args_invar_def reserved_regs_def by simp_all
+
+  show ?case
+  proof (cases rule: hIf_case[OF hIf.prems(2)])
+    case (1 z1 v1 z2)
+
+    obtain z1_c s2 where
+      ih1: "f_c \<turnstile> (to_imp_tc f_args crgt bs ?r1 stale t1, s) \<Rightarrow>\<^bsup>z1_c\<^esup>  s2" "s2 ?r1 = v1" "s = s2 on set stale - {?r1}"
+      using no_tails 1 args_invar rel_rgt rel_state1 hIf by metis
+
+    have rel_state2: "relate_exec_state f_args bs vs_arg vs_b s2"
+      using hIf ih1 unfolding relate_exec_state_def apply simp
+      unfolding map_eq_on_subset_eq[OF res_reg_subset(1)] map_eq_on_subset_eq[OF res_reg_subset(2)] by blast
+
+    obtain z2_c s3 where
+      ih2: "f_c \<turnstile> (to_imp_tc f_args crgt bs r stale t2, s2) \<Rightarrow>\<^bsup>z2_c\<^esup>  s3" "s3 r = v" "s2 = s3 on set stale - {r}"
+      using no_tails 1 args_invar rel_rgt rel_state2 hIf by metis
+
+    have "s = s2 on set stale - {r}" using ih1 fresh_not_in_stale eq_on_subset by blast
+    moreover have "s2 = s3 on set stale - {r}" using ih2 fresh_not_in_stale by auto
+    ultimately have s3_like_s: "s = s3 on set stale - {r}" by blast
+
+    show ?thesis apply (simp add: Let_def) apply (repeat \<open>rule exI\<close>; repeat \<open>rule conjI\<close>)
+        apply (rule tbig_step_t.tSeq) using ih1 apply blast apply (rule tbig_step_t.tIfTrue) using ih1 1 apply simp using ih2 apply simp apply simp apply simp
+        using ih2 apply simp using s3_like_s by auto
+  next
+    case (2 z1 z2)
+
+    obtain z1_c s2 where
+      ih1: "f_c \<turnstile> (to_imp_tc f_args crgt bs ?r1 stale t1, s) \<Rightarrow>\<^bsup>z1_c\<^esup>  s2" "s2 ?r1 = 0" "s = s2 on set stale - {?r1}"
+      using no_tails 2 args_invar rel_rgt rel_state1 hIf by metis
+
+    have rel_state2: "relate_exec_state f_args bs vs_arg vs_b s2"
+      using hIf ih1 unfolding relate_exec_state_def apply simp
+      unfolding map_eq_on_subset_eq[OF res_reg_subset(1)] map_eq_on_subset_eq[OF res_reg_subset(2)] by blast
+
+    obtain z2_c s3 where
+      ih2: "f_c \<turnstile> (to_imp_tc f_args crgt bs r stale t3, s2) \<Rightarrow>\<^bsup>z2_c\<^esup>  s3" "s3 r = v" "s2 = s3 on set stale - {r}"
+      using no_tails 2 args_invar rel_rgt rel_state2 hIf by metis
+
+    have "s = s2 on set stale - {r}" using ih1 fresh_not_in_stale eq_on_subset by blast
+    moreover have "s2 = s3 on set stale - {r}" using ih2 fresh_not_in_stale by auto
+    ultimately have s3_like_s: "s = s3 on set stale - {r}" by blast
+
+    show ?thesis apply (simp add: Let_def) apply (repeat \<open>rule exI\<close>; repeat \<open>rule conjI\<close>)
+        apply (rule tbig_step_t.tSeq) using ih1 apply blast apply (rule tbig_step_t.tIfFalse) using ih1 2 apply simp using ih2 apply simp apply simp apply simp
+        using ih2 apply simp using s3_like_s by auto
+  qed
+next
+  case (hCall gr ts)
+
+  obtain g T_g zs vs where
+          z: "z = sum_list zs + T_g vs"
+      and gr: "(g, T_g) = frgt gr"
+      and lengths: "length zs = length ts" "length vs = length ts"
+      and args_bigstep: "\<forall>i<length ts. (f, frgt) \<turnstile> (ts ! i, vs_b, vs_arg) \<Rightarrow>\<^bsup>zs ! i\<^esup> vs ! i"
+      and gvs: "g vs = v"
+    using hCall_case hCall by blast
+
+
+  let ?xs = "make_n_fresh stale ''Call.x.'' (length ts)"
+  let ?c1_gen = "\<lambda>crgt st. t_seqs' (map (\<lambda>i. to_imp_tc f_args crgt bs (?xs ! i) st (ts ! i)) [0..<length ts])"
+  let ?crgt_gen = "crgt(gr := (take (length ts) (args_from_crgt crgt gr), com_from_crgt crgt gr, ret_from_crgt crgt gr))"
+  let ?c1 = "?c1_gen crgt (?xs @ stale)"
+  let ?c2 = "t_seqs' (map (\<lambda>i. (args_from_crgt crgt gr ! i) ::= A (V (?xs ! i))) [0..<length ts])"
+  let ?c3 = "CALL com_from_crgt crgt gr RETURN ret_from_crgt crgt gr :: tcom"
+  let ?c4 = "r ::= A (V (ret_from_crgt crgt gr)) :: tcom"
+
+  (* let ?compiler_args_invar_weak = "\<lambda>f_args crgt bs stale t. *)
+        (* HOL_TCN_Timing.invar t *)
+        (* \<and> set (reserved_regs f_args crgt bs t) \<subseteq> set stale *)
+        (* \<and> distinct f_args *)
+        (* \<and> (\<forall>(g,_) \<in> set (calls t). distinct (args_from_crgt crgt g))" *)
+  (* from hCall(4) *)
+  (* have args_invar': "?compiler_args_invar_weak f_args crgt bs stale (hCall gr ts)" *)
+    (* unfolding compiler_args_invar_def by simp *)
+  have "\<exists>z1 s2. f_c \<turnstile> (?c1_gen crgt st,s) \<Rightarrow>\<^bsup>z1\<^esup> s2 \<and> lookups ?xs s2 = vs \<and> s = s2 on set stale"
+    if "set (?xs @ stale) \<subseteq> set st" "length ts = length (args_from_crgt crgt gr)" for st
+  using hCall(1,2,4,5,6) that args_bigstep proof (induction ts zs vs arbitrary: z v st crgt gr rule: snoc_list_induct3)
+    case Nil then show ?case unfolding make_n_fresh_def by auto
+  next
+    case (snoc ts_arg t_arg zs0 z0 vs0 v0)
+
+    let ?xs = "make_n_fresh stale ''Call.x.'' (length ts_arg)"
+    let ?xs' = "make_n_fresh stale ''Call.x.'' (length (ts_arg @ [t_arg]))"
+    let ?x = "make_nth_fresh stale ''Call.x.'' (length ts_arg)"
+    have xs': "?xs' = ?xs @ [?x]" unfolding make_n_fresh_def using nth_map_upt by simp
+    have x: "?xs' ! length ts_arg = ?x" unfolding xs' unfolding make_n_fresh_def by (subst nth_append) simp
+
+    let ?gr' = "fresh' (map fst (calls (hCall gr ts_arg))) ''g''"
+    (* let ?crgt = "crgt(?gr' := (take (length ts_arg) (args_from_crgt crgt gr), com_from_crgt crgt gr, ret_from_crgt crgt gr))" *)
+    let ?c1 = "t_seqs' (map (\<lambda>i. to_imp_tc f_args crgt bs (?xs ! i) st (ts_arg ! i)) [0..<length ts_arg])"
+    let ?c2 = "to_imp_tc f_args crgt bs ?x st t_arg"
+    term ?c1
+    (* have "set (calls (hCall gr ts_arg)) \<subseteq> set (calls (hCall gr (ts_arg @ [t_arg])))" *)
+      (* apply (induction ts_arg) apply auto *)
+    thm snoc
+    thm snoc.IH
+    have "\<exists>z1 s2. f_c \<turnstile> (?c1, s) \<Rightarrow>\<^bsup>z1\<^esup>  s2 \<and> lookups ?xs s2 = vs0 \<and> s = s2 on set stale"
+      apply (rule snoc.IH[where gr = gr]) (* ?gr' *)
+      subgoal using snoc.prems(1) by simp
+      subgoal using snoc.prems(2) by simp
+      subgoal
+        unfolding compiler_args_invar_def apply (repeat \<open>rule conjI\<close>)
+        subgoal using snoc.prems(3) unfolding compiler_args_invar_def by simp
+        subgoal using snoc.prems(3) unfolding compiler_args_invar_def reserved_regs_def thm set_take_subset apply simp done
+        subgoal using snoc.prems(3) unfolding compiler_args_invar_def by simp
+        subgoal using snoc.prems(3) unfolding compiler_args_invar_def by fastforce
+        subgoal using snoc.prems(3,7) unfolding compiler_args_invar_def apply (simp add: split_beta) sorry
+        done
+(* set (calls (hCall gr ts_arg) *)
+      subgoal using snoc.prems(4) unfolding relate_rgt_correctness_def by auto
+      subgoal using snoc.prems(5) by blast
+      subgoal using snoc.prems(6) unfolding make_n_fresh_def by fastforce
+      subgoal using snoc.prems(7) (* by (metis le_eq_less_or_eq le_imp_less_Suc length_append_singleton nth_append_left snoc.hyps(1,2)) *)
+        sorry
+      subgoal sorry
+      done
+    then obtain z1 s2 where ih1: "f_c \<turnstile> (?c1, s) \<Rightarrow>\<^bsup>z1\<^esup> s2" "lookups ?xs s2 = vs0" "s = s2 on set stale"
+      by blast
+
+
+    have t_arg_in_args: "t_arg \<in> set (ts_arg @ [t_arg])" by simp
+
+    have no_tails: "\<not> HOL_TCN_Timing.tails t_arg"
+      using that snoc.prems by auto
+
+    have calls_subset: "set (calls t_arg) \<subseteq> set (calls (hCall gr (ts_arg @ [t_arg])))"
+      using snoc.prems by auto
+
+    have args_invar: "compiler_args_invar f_args crgt bs st t_arg"
+    unfolding compiler_args_invar_def proof (repeat \<open>rule conjI\<close>)
+      show "HOL_TCN_Timing.invar t_arg" using no_tails_invar no_tails that by blast
+    next
+      have "set (reserved_regs f_args crgt bs t_arg) \<subseteq> set (reserved_regs f_args crgt bs (hCall gr (ts_arg @ [t_arg])))"
+        unfolding reserved_regs_def using calls_subset that by fastforce
+      then show "set (reserved_regs f_args crgt bs t_arg) \<subseteq> set st"
+        using snoc.prems unfolding compiler_args_invar_def by auto
+    next
+      show "distinct f_args" using hCall compiler_args_invar_def by simp
+    next
+      show "\<forall>(g,_)\<in>set (calls t_arg). distinct (args_from_crgt crgt g)"
+        using snoc.prems calls_subset that unfolding compiler_args_invar_def split_beta by blast
+    next
+      show "\<forall>(g, ts)\<in>set (calls t_arg). length ts = length (args_from_crgt crgt g)"
+        using snoc.prems calls_subset that unfolding compiler_args_invar_def split_beta by blast
+    qed
+
+    have rel_rgt: "relate_rgt_correctness frgt crgt (calls_r t_arg)"
+      using snoc.prems unfolding relate_rgt_correctness_def by auto
+
+    have exec_t_arg: "(f, frgt) \<turnstile> (t_arg, vs_b, vs_arg) \<Rightarrow>\<^bsup>z0\<^esup> v0" using snoc.prems
+      by (metis length_append_singleton lessI nth_append_length
+          snoc.hyps(1,2))
+
+    have "set f_args \<subseteq> set stale" "set bs \<subseteq> set stale"
+      using snoc.prems unfolding compiler_args_invar_def reserved_regs_def by simp_all
+    then have rel_state: "relate_exec_state f_args bs vs_arg vs_b s2" using snoc.prems(5) ih1
+      unfolding relate_exec_state_def using eq_on_subset by fastforce
+
+    obtain z2 s3 where texec_t_arg:
+        "f_c \<turnstile> (to_imp_tc f_args crgt bs ?x st t_arg, s2) \<Rightarrow>\<^bsup>z2\<^esup>  s3"
+        "s3 ?x = v0"
+        "s2 = s3 on set st - {?x}"
+      using snoc.prems t_arg_in_args no_tails exec_t_arg args_invar rel_rgt rel_state by metis
+    
+    show ?case proof (repeat \<open>rule exI\<close>; repeat \<open>rule conjI\<close>)
+      have "?x \<notin> set ?xs"
+        apply (subst sym[OF none_equal_not_in])
+        using make_n_fresh_def inj_on_contraD[OF inj_make_nth_fresh] by simp (* this should not be so hard... *)
+      then have "set ?xs \<subseteq> set (?xs' @ stale) - {?x}" using xs' fresh_not_in_stale unfolding make_nth_fresh_def by simp
+      also have "... \<subseteq> set st - {?x}" using snoc.prems by blast
+      finally show "lookups ?xs' s3 = vs0 @ [v0]"
+        using xs' ih1 texec_t_arg by fastforce
+    next
+      show "s = s3 on set stale"
+        using ih1 texec_t_arg fresh_not_in_stale make_nth_fresh_def snoc.prems(6) by fastforce
+    next
+      have 1: "map (\<lambda>i. to_imp_tc f_args crgt bs (?xs' ! i) st ((ts_arg @ [t_arg]) ! i)) [0..<length (ts_arg @ [t_arg])]
+        = map (\<lambda>i. to_imp_tc f_args crgt bs (?xs ! i) st (ts_arg ! i)) [0..<length ts_arg] @ [?c2]"
+        using xs' x unfolding make_n_fresh_def apply simp apply (subst nth_append)+ by simp
+
+      thm t_seqs'_append
+      have "f_c \<turnstile> (?c1;; ?c2,s) \<Rightarrow>\<^bsup>z1 + z2\<^esup> s3" using ih1 texec_t_arg tbig_step_t.tSeq by blast
+      then have "f_c \<turnstile> (t_seqs' (map (\<lambda>i. to_imp_tc f_args crgt bs (?xs ! i) st (ts_arg ! i)) [0..<length ts_arg] @ [?c2]),s) \<Rightarrow>\<^bsup>z1 + z2\<^esup>  s3"
+        apply (subst t_seqs'_append[symmetric]) apply (subst (2) t_seqs_def) apply simp apply (subst tbig_step_t_tSeq_assoc) using tbig_step_t.tSeq by fastforce
+      with 1 show "f_c \<turnstile> (t_seqs' (map (\<lambda>i. to_imp_tc f_args crgt bs (?xs' ! i) st ((ts_arg @ [t_arg]) ! i)) [0..<length (ts_arg @ [t_arg])]),s) \<Rightarrow>\<^bsup>z1 + z2\<^esup>  s3"
+        by metis
+    qed
+  qed (simp_all add: lengths)
+
+  moreover have lll: "length ts = length (args_from_crgt crgt gr)"
+    using hCall.prems unfolding compiler_args_invar_def by simp
+  ultimately obtain z1 s2 where exec_c1: "f_c \<turnstile> (?c1,s) \<Rightarrow>\<^bsup>z1\<^esup> s2" and "lookups ?xs s2 = vs" and s2: "s = s2 on set stale"
+    using hCall.prems unfolding compiler_args_invar_def by blast
+
+
+  (* part 2: copying from temporaries to argument registers *)
+
+  have lll2: "length ?xs = length (args_from_crgt crgt gr)"
+    using lll unfolding make_n_fresh_def by simp
+
+  have "set (args_from_crgt crgt gr) \<subseteq> set stale"
+    using hCall.prems unfolding compiler_args_invar_def reserved_regs_def by simp
+  then have ddd: "distinct (?xs @ args_from_crgt crgt gr)"
+    apply simp using hCall.prems make_n_fresh_not_in_stale unfolding compiler_args_invar_def apply simp
+    apply (rule Int_emptyI) by blast
+
+  thm copy_list_sem
+  thm copy_list_sem[where s = s2 and f = f_c and xs = ?xs and ys = "args_from_crgt crgt gr", OF lll2 ddd]
+
+  obtain s3 where "f_c \<turnstile> (t_seqs'
+               (map (\<lambda>i. (args_from_crgt crgt gr ! i) ::= A (V (make_n_fresh stale ''Call.x.'' (length ts) ! i)))
+                 [0..<length (make_n_fresh stale ''Call.x.'' (length ts))]),
+              s2) \<Rightarrow>\<^bsup>Suc (2 * length (make_n_fresh stale ''Call.x.'' (length ts)))\<^esup>  s3"
+      "lookups ?xs s2 = lookup_args crgt gr s3 " and s3: "s2 = s3 on - set (args_from_crgt crgt gr)"
+    using copy_list_sem[OF lll2 ddd] by blast
+  then obtain z2 where exec_c2: "f_c \<turnstile> (?c2, s2) \<Rightarrow>\<^bsup>z2\<^esup> s3"
+    unfolding make_n_fresh_def by simp
+
+
+  (* part 3: calling g *)
+
+  let ?gcom = "com_from_crgt crgt gr" and ?gret = "ret_from_crgt crgt gr" and ?gv = "f_from_frgt frgt gr (lookup_args crgt gr s3)"
+  have "terminates_with_res_IMP ?gcom s3 ?gret ?gv" using hCall.prems unfolding relate_rgt_correctness_def by simp
+  then obtain z3 s4c where "(?gcom, s3) \<Rightarrow>\<^bsup>z3\<^esup> s4c" "s4c ?gret = ?gv"
+    unfolding terminates_with_res_IMP_def terminates_with_res_pred_time_IMP_def terminates_with_pred_time_IMP_def by blast
+  then obtain s4 where exec_c3: "f_c \<turnstile> (?c3, s3) \<Rightarrow>\<^bsup>z3\<^esup> s4" and s4: "s4 = s3(?gret := ?gv)" using tbig_step_t.tCall by fastforce
+
+  have vfrom: "v = f_from_frgt frgt gr (lookup_args crgt gr s3)"
+    by (metis \<open>(g, T_g) = frgt gr\<close> \<open>g vs = v\<close> \<open>lookups ?xs s2 = lookup_args crgt gr s3\<close>
+        \<open>lookups ?xs s2 = vs\<close> fst_conv) (* TODO clean *)
+
+
+  (* part 4: copying to r *)
+
+  term ?c4
+  let ?s5 = "s4(r := aval (A (V ?gret)) s4)"
+  obtain z4 where exec_c4: "f_c \<turnstile> (?c4, s4) \<Rightarrow>\<^bsup>z4\<^esup> ?s5" by blast
+  then have s5: "?s5 = s4(r := v)" using vfrom s4 by simp
+
+
+  (* putting it together *)
+
+  have "f_c \<turnstile> (?c1;; ?c2;; ?c3;; ?c4, s) \<Rightarrow>\<^bsup>z1 + z2 + z3 + z4\<^esup> ?s5"
+    using exec_c1 exec_c2 exec_c3 exec_c4 by blast
+
+  have "?s5 r = v" using s5 by simp
+
+  have "s = s2 on set stale" using s2 .
+  have "set stale \<subseteq> - set (args_from_crgt crgt gr)"
+    using hCall.prems unfolding compiler_args_invar_def reserved_regs_def 
+(* not equal on all of stale! have to fix lemma *) sorry
+  have "s2 = s3 on set stale" using s3 using hCall.prems unfolding compiler_args_invar_def reserved_regs_def 
+  have "s = ?s5 on set stale - {r}" using s2 s3 s4 s5 apply simp
+  
+
+  thm hCall_case[OF hCall.prems(2)]
+  have ?case
+  apply (simp only: to_imp_tc.simps Let_def split_beta mapi_map cc_call_helper[symmetric])
+  proof (repeat \<open>rule exI\<close>; repeat \<open>rule conjI\<close>)
+    apply (subst sym[OF cc_call_helper]) sorry
+
+
+
+  have tsi_in_ts: "ts ! i \<in> set ts" if "i < length ts" for i using that by simp
+  (* have 8: "P (ts ! i)" if "i < length ts" "\<forall>t\<in>set ts. P t" for P i using that by auto *)
+
+  have no_tails: "\<not> HOL_TCN_Timing.tails (ts ! i)" if "i < length ts" for i using hCall that by auto
+
+  have calls_subset: "set (calls (ts ! i)) \<subseteq> set (calls (hCall gr ts))" if "i < length ts" for i using hCall tsi_in_ts that by fastforce
+
+  have args_invar: "compiler_args_invar f_args crgt bs stale (ts ! i)" if "i < length ts" for i
+  unfolding compiler_args_invar_def proof (repeat \<open>rule conjI\<close>)
+    show "HOL_TCN_Timing.invar (ts ! i)" using no_tails_invar no_tails that by blast
+  next
+    have "set (reserved_regs f_args crgt bs (ts ! i)) \<subseteq> set (reserved_regs f_args crgt bs (hCall gr ts))"
+      unfolding reserved_regs_def using calls_subset that by fastforce
+    then show "set (reserved_regs f_args crgt bs (ts ! i)) \<subseteq> set stale"
+      using hCall unfolding compiler_args_invar_def by auto
+  next
+    show "distinct f_args" using hCall compiler_args_invar_def by simp
+  next
+    show "\<forall>g\<in>set (calls (ts ! i)). distinct (args_from_crgt crgt g)"
+      using hCall calls_subset that unfolding compiler_args_invar_def by blast
+  qed
+
+  
+(* 
+  have no_tails: "\<not> HOL_TCN_Timing.tails (ts ! i)"
+    and args_invar: "compiler_args_invar f_args crgt bs stale (ts ! i)"
+    (* and "set (calls (ts ! i)) \<subseteq> set (calls (hCall gr ts))" *)
+    if "i < length ts" for i
+    (* using hCall tsi_in_ts that by auto *)
+  proof (goal_cases)
+    case 1 then show ?case using hCall tsi_in_ts that by auto
+  next
+    case 2
+    then show ?case sorry
+  qed
+    show "\<not> HOL_TCN_Timing.tails (ts ! i)"
+    (* have tsi_in_ts: "ts ! i \<in> set ts" using that by simp *)
+    
+
+  have "set (calls (ts ! i)) \<subseteq> set (calls (hCall gr ts))" if "i < length ts" for i using hCall tsi_in_ts that by fastforce
+  then have args_invar: "compiler_args_invar f_args crgt bs stale (ts ! i)" if "i < length ts" for i
+    using hCall tsi_in_ts that unfolding compiler_args_invar_def reserved_regs_def apply simp
+
+  show ?case
+    apply (simp add: Let_def split_beta mapi_map del: One_nat_def) *)
+    
+    sorry (* TODO :< *)
+next
+  case (hTAIL x)
+  then show ?case by simp
+qed
 
 
 (*
@@ -197,17 +724,17 @@ thm tto_end_non_tail tto_end_tail *)
 find_theorems "map fst"
 lemma
   assumes compiler_correct_nt_: True
-  fixes t_imp f_args ctxt reg bs r stale t vs_b vs_arg
-  defines "t_imp \<equiv> to_imp_tc f_args ctxt bs r stale t"
-  assumes "t_time \<equiv> time_to_tail reg vs_b vs_arg t"
-  assumes "well_formed_comp f_args ctxt bs stale t"
+  fixes t_imp f_args crgt frgt bs r stale t vs_b vs_arg
+  defines "t_imp \<equiv> to_imp_tc f_args crgt bs r stale t"
+  assumes "t_time \<equiv> time_to_tail frgt vs_b vs_arg t"
+  assumes "well_formed_comp f_args crgt bs stale t"
   assumes "well_encoded_comp f_args bs vs_arg vs_b s"
-  (* assumes "called_correctness ctxt reg t" *)
+  (* assumes "called_correctness crgt frgt t" *)
   shows "\<exists>k Cs.
     (\<exists>t l. tto_end s t_imp k Cs t l)
     \<and> length Cs = length t_time
     \<and> (\<forall>((C,s), (g,vs_arg_g)) \<in> set (zip Cs t_time).
-          C = com_from_ctxt ctxt g \<and> vs_arg_g = lookup_args ctxt g s)"
+          C = com_from_crgt crgt g \<and> vs_arg_g = lookup_args crgt g s)"
 using assms(2-4) proof (induction t arbitrary: t_imp t_time bs r stale vs_b s)
   case (hLet t1 t2)
   then show ?case sorry
@@ -226,14 +753,14 @@ next
 next
   case (hCall g ts)
   let ?xs = "make_n_fresh (length ts) stale ''Call.x.''"
-  let ?cs1 = "mapi (\<lambda>i t. to_imp_tc f_args ctxt bs (?xs ! i) (?xs @ stale) t) ts"
-  let ?cs2 = "mapi (\<lambda>i t. tAssign (args_from_ctxt ctxt g ! i) (A (V (?xs ! i)))) ts"
-  let ?call = "tSeq (tCall (com_from_ctxt ctxt g) (ret_from_ctxt ctxt g)) (tAssign r (A (V (ret_from_ctxt ctxt g))))"
+  let ?cs1 = "mapi (\<lambda>i t. to_imp_tc f_args crgt bs (?xs ! i) (?xs @ stale) t) ts"
+  let ?cs2 = "mapi (\<lambda>i t. tAssign (args_from_crgt crgt g ! i) (A (V (?xs ! i)))) ts"
+  let ?call = "tSeq (tCall (com_from_crgt crgt g) (ret_from_crgt crgt g)) (tAssign r (A (V (ret_from_crgt crgt g))))"
 
   have "t_imp = t_seqs (?cs1 @ ?cs2) ?call" using hCall by (simp add: Let_def split_beta)
 
-  let ?x = "\<lambda>s. f_from_reg reg g (lookup_args ctxt g s)"
-  have "tto_end s ?call 2 [(com_from_ctxt ctxt g,s)] (s(ret_from_ctxt ctxt g := ?x s, r := ?x s)) False" for s
+  let ?x = "\<lambda>s. f_from_reg frgt g (lookup_args crgt g s)"
+  have "tto_end s ?call 2 [(com_from_crgt crgt g,s)] (s(ret_from_crgt crgt g := ?x s, r := ?x s)) False" for s
     sorry
 
   then show ?case sorry
@@ -245,21 +772,21 @@ qed
 
 
 
-    (* \<and> (\<forall>((C,s), (g,vs_arg_g)) \<in> set (zip gs (time_to_tail reg vs_b vs_arg t)). *)
-          (* C = com_from_ctxt ctxt g \<and> vs_arg_g = lookup_args ctxt g s)" *)
+    (* \<and> (\<forall>((C,s), (g,vs_arg_g)) \<in> set (zip gs (time_to_tail frgt vs_b vs_arg t)). *)
+          (* C = com_from_crgt crgt g \<and> vs_arg_g = lookup_args crgt g s)" *)
 
 *)
 
 lemma
   assumes compiler_correct_nt_: True
-  assumes "t_imp = to_imp_tc f_args ctxt bs r stale t"
-  assumes "well_formed_comp f_args ctxt bs stale t"
+  assumes "t_imp = to_imp_tc f_args crgt bs r stale t"
+  assumes "well_formed_comp f_args crgt bs stale t"
   assumes "well_encoded_comp f_args bs vs_arg vs_b s"
-  assumes "called_correctness ctxt reg t"
+  assumes "called_correctness crgt frgt t"
   shows "\<exists>k z.
     ttime_to_tail s t_imp (k + z)
     \<and> k \<le> tstruct_k t_imp
-    \<and> z \<le> tinterp_time reg ctxt (time_to_tail reg vs_b vs_arg t)"
+    \<and> z \<le> tinterp_time frgt crgt (time_to_tail frgt vs_b vs_arg t)"
 using assms(2-5) proof (induction t arbitrary: t_imp bs r stale vs_b s)
   case (hLet t1 t2)
   thm hLet.prems(1)[simplified]
@@ -268,15 +795,15 @@ using assms(2-5) proof (induction t arbitrary: t_imp bs r stale vs_b s)
   thm hLet.prems
 
   let ?x_var = "fresh' stale ''Let.x''"
-  let ?t_imp1 = "to_imp_tc f_args ctxt bs ?x_var stale t1"
+  let ?t_imp1 = "to_imp_tc f_args crgt bs ?x_var stale t1"
 
-  have wf1: "well_formed_comp f_args ctxt bs stale t1" using hLet.prems(2)
+  have wf1: "well_formed_comp f_args crgt bs stale t1" using hLet.prems(2)
     unfolding well_formed_comp_def using non_tail_tailrec apply auto apply (simp only: reserved_regs_def h_calls.simps map_append)
     by auto
   then obtain k1 z1 where k1z1:
       "ttime_to_tail s ?t_imp1 (k1 + z1)"
       "k1 \<le> tstruct_k ?t_imp1"
-      "z1 \<le> tinterp_time reg ctxt (time_to_tail reg vs_b vs_arg t1)"
+      "z1 \<le> tinterp_time frgt crgt (time_to_tail frgt vs_b vs_arg t1)"
     using hLet.IH(1)[where t_imp = ?t_imp1 and s = s and bs = bs and vs_b = vs_b and r = ?x_var and stale = stale] hLet.prems
     unfolding called_correctness_def by auto
 
@@ -284,7 +811,7 @@ using assms(2-5) proof (induction t arbitrary: t_imp bs r stale vs_b s)
   have ob2: "well_encoded_comp f_args bs vs_arg vs_b s" using hLet by simp
   obtain f y1 s1
       where t1s1: "f \<turnstile> (?t_imp1,s) \<Rightarrow>\<^bsup>y1\<^esup> s1"
-      and s1_xvar: "s1 ?x_var = eval_non_tail reg vs_b vs_arg t1"
+      and s1_xvar: "s1 ?x_var = eval_non_tail frgt vs_b vs_arg t1"
       and s1: "s = s1 on (Set.remove ?x_var (set stale))"
     using compiler_correct_nt[OF ob1 wf1 ob2, simplified] by blast
 
@@ -292,10 +819,10 @@ using assms(2-5) proof (induction t arbitrary: t_imp bs r stale vs_b s)
   then have inv: "invar ?t_imp1" using to_imp_invar by blast
   have y1: "y1 = k1 + z1" using ttime_non_tail[OF inv t1s1] sorry (* ttime_to_tail for non-tail MUST INVESTIGATE AND WRITE LEMMA *)
 
-  let ?t_imp2 = "to_imp_tc f_args ctxt (?x_var # bs) r (?x_var # stale) t2"
+  let ?t_imp2 = "to_imp_tc f_args crgt (?x_var # bs) r (?x_var # stale) t2"
   have "tailrec t2" using hLet unfolding well_formed_comp_def by simp
 
-  have t2_1: "well_formed_comp f_args ctxt (?x_var # bs) (?x_var # stale) t2"
+  have t2_1: "well_formed_comp f_args crgt (?x_var # bs) (?x_var # stale) t2"
     using hLet.prems(2) unfolding well_formed_comp_def apply auto sorry (* almost sub-term *)
   have "set f_args \<subseteq> Set.remove ?x_var (set stale)" using fresh_not_in_stale
     unfolding remove_def apply simp using hLet.prems(2) unfolding well_formed_comp_def reserved_regs_def by simp
@@ -304,26 +831,26 @@ using assms(2-5) proof (induction t arbitrary: t_imp bs r stale vs_b s)
     using s1 apply blast using hLet.prems(3) unfolding well_encoded_comp_def by blast
   have "set bs \<subseteq> Set.remove ?x_var (set stale)" using fresh_not_in_stale
     unfolding remove_def apply simp using hLet.prems(2) unfolding well_formed_comp_def reserved_regs_def by simp
-  then have t2_2_2: "lookups (?x_var # bs) s1 = eval_non_tail reg vs_b vs_arg t1 # vs_b" apply auto
+  then have t2_2_2: "lookups (?x_var # bs) s1 = eval_non_tail frgt vs_b vs_arg t1 # vs_b" apply auto
     using s1_xvar apply blast
     apply (subst lookups_eq_on[where s = s, symmetric])
     using s1 apply blast using hLet.prems(3) unfolding well_encoded_comp_def by blast
-  from t2_2_1 t2_2_2 have t2_2: "well_encoded_comp f_args (?x_var # bs) vs_arg (eval_non_tail reg vs_b vs_arg t1 # vs_b) s1"
+  from t2_2_1 t2_2_2 have t2_2: "well_encoded_comp f_args (?x_var # bs) vs_arg (eval_non_tail frgt vs_b vs_arg t1 # vs_b) s1"
     unfolding well_encoded_comp_def by simp
-  have t2_3: "called_correctness ctxt reg t2" using hLet.prems(4) unfolding called_correctness_def by auto
+  have t2_3: "called_correctness crgt frgt t2" using hLet.prems(4) unfolding called_correctness_def by auto
   obtain k2 z2 where k2z2:
       "ttime_to_tail s1 ?t_imp2 (k2 + z2)"
       "k2 \<le> tstruct_k ?t_imp2"
-      "z2 \<le> tinterp_time reg ctxt (time_to_tail reg (eval_non_tail reg vs_b vs_arg t1 # vs_b) vs_arg t2)"
+      "z2 \<le> tinterp_time frgt crgt (time_to_tail frgt (eval_non_tail frgt vs_b vs_arg t1 # vs_b) vs_arg t2)"
     using hLet.IH(2)[where t_imp = ?t_imp2 and r = r and s = s1 and bs = "?x_var # bs"
-      and vs_b = "eval_non_tail reg vs_b vs_arg t1 # vs_b" and stale = "?x_var # stale", OF _ t2_1 t2_2 t2_3, simplified]
+      and vs_b = "eval_non_tail frgt vs_b vs_arg t1 # vs_b" and stale = "?x_var # stale", OF _ t2_1 t2_2 t2_3, simplified]
     by blast
 
   from t1s1 k2z2
   have "ttime_to_tail s t_imp (y1 + (k2 + z2))" using hLet.prems(1) apply simp unfolding Let_def apply (rule ttime_to_tail.intros(3)) by auto
   moreover have "y1 + (k2 + z2) = (k1 + k2) + (z1 + z2)" using y1 by linarith
   moreover have "k1 + k2 \<le> tstruct_k t_imp" using hLet.prems(1) apply simp unfolding Let_def using k1z1 k2z2 by simp
-  moreover have "z1 + z2 \<le> tinterp_time reg ctxt (time_to_tail reg vs_b vs_arg (hLet t1 t2))"
+  moreover have "z1 + z2 \<le> tinterp_time frgt crgt (time_to_tail frgt vs_b vs_arg (hLet t1 t2))"
     apply simp using k1z1 k2z2 unfolding tinterp_time_def by simp
 
   ultimately show ?case by auto
@@ -367,7 +894,7 @@ next
   then show ?case sorry
 qed
 
-lemma "\<exists>c. \<forall>s. tstruct_k t_imp + something \<le> c * interp_time reg (time_to_tail reg vs_b vs_arg t)" oops
+lemma "\<exists>c. \<forall>s. tstruct_k t_imp + something \<le> c * interp_time frgt (time_to_tail frgt vs_b vs_arg t)" oops
 (* in fact, we can calculate c as the max of the structural-constant-factor and all T_f_const-ants or so *)
 
 end
