IMP/HOL_TCN_Timing.thy
@@ -31,58 +31,49 @@ notation hLet ("LET _ IN _") and
          hIf ("(IF _/\<noteq>0 THEN _/ ELSE _)"  [0, 0, 61] 61)
 end
 
+(* find_consts "('a \<Rightarrow> 'b set) \<Rightarrow> 'b set" *)
 
+(* TODO: could maybe return a set *)
 fun calls where
   "calls (LET t1 IN t2) = calls t1 @ calls t2" |
   "calls (hLetBound _) = []" |
   "calls (hArg _) = []" |
   "calls (hNumber _) = []" |
   "calls (IF t1\<noteq>0 THEN t2 ELSE t3) = calls t1 @ calls t2 @ calls t3" |
-  "calls (hCall f ts) = f # concat (map calls ts)" |
+  "calls (hCall f ts) = (f, ts) # concat (map calls ts)" |
   "calls (hTAIL ts) = concat (map calls ts)"
 
-
 (* function name \<Rightarrow> (function \<times> timing function) *)
-type_synonym thol_reg = "fun_ref \<Rightarrow> ((nat list \<Rightarrow> nat) \<times> (nat list \<Rightarrow> nat))"
-abbreviation "f_from_reg (reg :: thol_reg) name \<equiv> fst (reg name)"
-abbreviation "T_f_from_reg (reg :: thol_reg) name \<equiv> snd (reg name)"
+type_synonym fun_registry = "fun_ref \<Rightarrow> ((nat list \<Rightarrow> nat) \<times> (nat list \<Rightarrow> nat))"
+abbreviation "f_from_frgt (frgt :: fun_registry) name \<equiv> fst (frgt name)"
+abbreviation "T_f_from_frgt (frgt :: fun_registry) name \<equiv> snd (frgt name)"
 
-lemma split_from_reg:
-  "(f, T_f) = reg fr \<longleftrightarrow> f_from_reg reg fr = f \<and> T_f_from_reg reg fr = T_f"
+lemma split_from_frgt:
+  "(f, T_f) = frgt fr \<longleftrightarrow> f_from_frgt frgt fr = f \<and> T_f_from_frgt frgt fr = T_f"
   using split_pairs .
-
-(* function name \<Rightarrow> (argument registers' names \<times> IMP command \<times> return register's name *)
-type_synonym thol_ctxt = "fun_ref \<Rightarrow> (vname list \<times> com \<times> vname)"
-abbreviation "args_from_ctxt (ctxt :: thol_ctxt) name \<equiv> fst (ctxt name)"
-abbreviation "com_from_ctxt (ctxt :: thol_ctxt) name \<equiv> fst (snd (ctxt name))"
-abbreviation "ret_from_ctxt (ctxt :: thol_ctxt) name \<equiv> snd (snd (ctxt name))"
-(* TODO: use these abbrev. *)
-(* TODO: use better names than reg/ctxt *)
-
-definition "null = (\<lambda>_. undefined)"
 
 
 inductive
-  hbig_step_t :: "thol \<times> thol_reg \<Rightarrow> thol \<times> nat list \<times> nat list \<Rightarrow> nat \<Rightarrow> nat \<Rightarrow> bool" ("_ \<turnstile> _ \<Rightarrow>\<^bsup>_\<^esup>  _" 55)
+  hbig_step_t :: "thol \<times> fun_registry \<Rightarrow> thol \<times> nat list \<times> nat list \<Rightarrow> nat \<Rightarrow> nat \<Rightarrow> bool" ("_ \<turnstile> _ \<Rightarrow>\<^bsup>_\<^esup>  _" 55)
   where
 hLet: "\<lbrakk>env \<turnstile> (t1,bs,xs) \<Rightarrow>\<^bsup>z1\<^esup> v1; env \<turnstile> (t2,v1#bs,xs) \<Rightarrow>\<^bsup>z2\<^esup> v; z = z1+z2\<rbrakk>
        \<Longrightarrow> env \<turnstile> (LET t1 IN t2,bs,xs) \<Rightarrow>\<^bsup>z\<^esup> v" |
-hLetBound: "v = bs!n \<Longrightarrow> env \<turnstile> (hLetBound n,bs,xs) \<Rightarrow>\<^bsup>0\<^esup> v" |
-hArg: "v = xs!n \<Longrightarrow> env \<turnstile> (hArg n,bs,xs) \<Rightarrow>\<^bsup>0\<^esup> v" |
+hLetBound: "n < length bs \<Longrightarrow> env \<turnstile> (hLetBound n,bs,xs) \<Rightarrow>\<^bsup>0\<^esup> bs!n" |
+hArg: "n < length xs \<Longrightarrow> env \<turnstile> (hArg n,bs,xs) \<Rightarrow>\<^bsup>0\<^esup> xs!n" |
 hNumber: "env \<turnstile> (hNumber n,bs,xs) \<Rightarrow>\<^bsup>0\<^esup> n" |
 hIfTrue: "\<lbrakk>env \<turnstile> (t1,bs,xs) \<Rightarrow>\<^bsup>z1\<^esup> v1; v1 \<noteq> 0; env \<turnstile> (t2,bs,xs) \<Rightarrow>\<^bsup>z2\<^esup> v2; z = z1+z2\<rbrakk>
           \<Longrightarrow> env \<turnstile> (IF t1\<noteq>0 THEN t2 ELSE t3,bs,xs) \<Rightarrow>\<^bsup>z\<^esup> v2" |
 hIfFalse: "\<lbrakk>env \<turnstile> (t1,bs,xs) \<Rightarrow>\<^bsup>z1\<^esup> v1; v1 = 0; env \<turnstile> (t3,bs,xs) \<Rightarrow>\<^bsup>z2\<^esup> v2; z = z1+z2\<rbrakk>
           \<Longrightarrow> env \<turnstile> (IF t1\<noteq>0 THEN t2 ELSE t3,bs,xs) \<Rightarrow>\<^bsup>z\<^esup> v2" |
-hCall: "\<lbrakk>(g, T_g) = reg gr; length zs = length ts; length vs = length ts;
-          \<forall>i < length ts. (f,reg) \<turnstile> (ts ! i, bs, xs) \<Rightarrow>\<^bsup>zs ! i\<^esup> vs ! i;
+hCall: "\<lbrakk>(g, T_g) = frgt gr; length zs = length ts; length vs = length ts;
+          \<forall>i < length ts. (f,frgt) \<turnstile> (ts ! i, bs, xs) \<Rightarrow>\<^bsup>zs ! i\<^esup> vs ! i;
           g vs = v'; z' = sum_list zs + T_g vs\<rbrakk>
-          \<Longrightarrow> (f,reg) \<turnstile> (hCall gr ts,bs,xs) \<Rightarrow>\<^bsup>z'\<^esup> v'" |
+          \<Longrightarrow> (f,frgt) \<turnstile> (hCall gr ts,bs,xs) \<Rightarrow>\<^bsup>z'\<^esup> v'" |
 hTAIL: "\<lbrakk>length zs = length ts; length vs = length ts;
-          \<forall>i < length ts. (f,reg) \<turnstile> (ts ! i, bs, xs) \<Rightarrow>\<^bsup>zs ! i\<^esup> vs ! i;
-          (f,reg) \<turnstile> (f,[],vs) \<Rightarrow>\<^bsup>z'\<^esup> v';
+          \<forall>i < length ts. (f,frgt) \<turnstile> (ts ! i, bs, xs) \<Rightarrow>\<^bsup>zs ! i\<^esup> vs ! i;
+          (f,frgt) \<turnstile> (f,[],vs) \<Rightarrow>\<^bsup>z'\<^esup> v';
           z'' = sum_list zs + z' + 1\<rbrakk>
-          \<Longrightarrow> (f,reg) \<turnstile> (hTAIL ts,bs,xs) \<Rightarrow>\<^bsup>z''\<^esup> v'"
+          \<Longrightarrow> (f,frgt) \<turnstile> (hTAIL ts,bs,xs) \<Rightarrow>\<^bsup>z''\<^esup> v'"
 
 print_theorems
 
@@ -95,8 +86,8 @@ inductive_cases hLetBound_case [elim!]: "env \<turnstile> (hLetBound n,bs,xs) \<
 inductive_cases hArg_case [elim!]: "env \<turnstile> (hArg n,bs,xs) \<Rightarrow>\<^bsup>z\<^esup> v"
 inductive_cases hNumber_case [elim!]: "env \<turnstile> (hNumber n,bs,xs) \<Rightarrow>\<^bsup>z\<^esup> v"
 inductive_cases hIf_case [elim!]: "env \<turnstile> (hIf t1 t2 t3,bs,xs) \<Rightarrow>\<^bsup>z\<^esup> v"
-inductive_cases hCall_case [elim!]: "(f,reg) \<turnstile> (hCall g ts,bs,xs) \<Rightarrow>\<^bsup>z\<^esup> v"
-inductive_cases hTAIL_case [elim!]: "(f,reg) \<turnstile> (hTAIL ts,bs,xs) \<Rightarrow>\<^bsup>z\<^esup> v"
+inductive_cases hCall_case [elim!]: "(f,frgt) \<turnstile> (hCall g ts,bs,xs) \<Rightarrow>\<^bsup>z\<^esup> v"
+inductive_cases hTAIL_case [elim!]: "(f,frgt) \<turnstile> (hTAIL ts,bs,xs) \<Rightarrow>\<^bsup>z\<^esup> v"
 lemmas hbig_step_t_cases = hLet_case hLetBound_case hArg_case hNumber_case hIf_case hCall_case hTAIL_case
 
 
@@ -107,7 +98,7 @@ lemma determ:
   shows "z1 = z2" "v1 = v2"
   oops (* TODO *)
 (* using assms proof (induction arbitrary: z2 v2 rule: hbig_step_t.induct)
-  case (hCall g T_g reg gr zs ts vs f bs xs v' z')
+  case (hCall g T_g frgt gr zs ts vs f bs xs v' z')
   {
     case 1
     then show ?case sorry (* TODO *)
@@ -116,7 +107,7 @@ lemma determ:
     then show ?case sorry
   }
 next
-  case (hTAIL zs ts vs f reg bs xs z' v' z'')
+  case (hTAIL zs ts vs f frgt bs xs z' v' z'')
   {
     case 1
     then show ?case sorry
@@ -148,43 +139,43 @@ lemma no_tails_invar[simp]: "\<not> tails t \<Longrightarrow> invar t" by (induc
 
 type_synonym trace = "(fun_ref \<times> nat list) list"
 
-definition "interp_trace_item reg g vs_arg_g = T_f_from_reg reg g vs_arg_g"
-definition "interp_trace reg = sum_map (\<lambda>(g, vs_arg_g). interp_trace_item reg g vs_arg_g)"
+definition "interp_trace_item frgt g vs_arg_g = T_f_from_frgt frgt g vs_arg_g"
+definition "interp_trace frgt = sum_map (\<lambda>(g, vs_arg_g). interp_trace_item frgt g vs_arg_g)"
 
 lemma interp_trace_append[simp]:
-  "interp_trace reg (xs @ ys) = interp_trace reg xs + interp_trace reg ys"
+  "interp_trace frgt (xs @ ys) = interp_trace frgt xs + interp_trace frgt ys"
   unfolding interp_trace_def by simp
 lemma interp_trace_concat_is_sum_map:
-  "interp_trace reg (concat xss) = sum_map (interp_trace reg) xss"
+  "interp_trace frgt (concat xss) = sum_map (interp_trace frgt) xss"
   unfolding interp_trace_def by (induction xss) auto
 
 datatype leaf_state = Value nat | Tail "nat list"
 
 inductive
-  htrace_to_leaf :: "thol_reg \<Rightarrow> thol \<times> nat list \<times> nat list \<Rightarrow> trace \<Rightarrow> leaf_state \<Rightarrow> bool"  ("_ \<turnstile> _ \<Rightarrow>\<^bsup>_\<^esup>  _" 55)
+  htrace_to_leaf :: "fun_registry \<Rightarrow> thol \<times> nat list \<times> nat list \<Rightarrow> trace \<Rightarrow> leaf_state \<Rightarrow> bool"  ("_ \<turnstile> _ \<Rightarrow>\<^bsup>_\<^esup>  _" 55)
 where
 hLet:
-  "\<lbrakk>reg \<turnstile> (t1,bs,xs) \<Rightarrow>\<^bsup>T1\<^esup> Value v1; reg \<turnstile> (t2,v1#bs,xs) \<Rightarrow>\<^bsup>T2\<^esup> l2; T = T1@T2\<rbrakk>
-   \<Longrightarrow> reg \<turnstile> (LET t1 IN t2,bs,xs) \<Rightarrow>\<^bsup>T\<^esup> l2" |
-hLetBound: "reg \<turnstile> (hLetBound n,bs,xs) \<Rightarrow>\<^bsup>[]\<^esup> Value (bs ! n)" |
-hArg: "reg \<turnstile> (hArg n,bs,xs) \<Rightarrow>\<^bsup>[]\<^esup> Value (xs ! n)" |
-hNumber: "reg \<turnstile> (hNumber n,bs,xs) \<Rightarrow>\<^bsup>[]\<^esup> Value n" |
+  "\<lbrakk>frgt \<turnstile> (t1,bs,xs) \<Rightarrow>\<^bsup>T1\<^esup> Value v1; frgt \<turnstile> (t2,v1#bs,xs) \<Rightarrow>\<^bsup>T2\<^esup> l2; T = T1@T2\<rbrakk>
+   \<Longrightarrow> frgt \<turnstile> (LET t1 IN t2,bs,xs) \<Rightarrow>\<^bsup>T\<^esup> l2" |
+hLetBound: "n < length bs \<Longrightarrow> frgt \<turnstile> (hLetBound n,bs,xs) \<Rightarrow>\<^bsup>[]\<^esup> Value (bs ! n)" |
+hArg: "n < length xs \<Longrightarrow> frgt \<turnstile> (hArg n,bs,xs) \<Rightarrow>\<^bsup>[]\<^esup> Value (xs ! n)" |
+hNumber: "frgt \<turnstile> (hNumber n,bs,xs) \<Rightarrow>\<^bsup>[]\<^esup> Value n" |
 hIfTrue:
-  "\<lbrakk>reg \<turnstile> (t1,bs,xs) \<Rightarrow>\<^bsup>T1\<^esup> Value v1; v1 \<noteq> 0; reg \<turnstile> (t2,bs,xs) \<Rightarrow>\<^bsup>T2\<^esup> l2; T = T1@T2\<rbrakk>
-   \<Longrightarrow> reg \<turnstile> (IF t1\<noteq>0 THEN t2 ELSE t3,bs,xs) \<Rightarrow>\<^bsup>T\<^esup> l2" |
+  "\<lbrakk>frgt \<turnstile> (t1,bs,xs) \<Rightarrow>\<^bsup>T1\<^esup> Value v1; v1 \<noteq> 0; frgt \<turnstile> (t2,bs,xs) \<Rightarrow>\<^bsup>T2\<^esup> l2; T = T1@T2\<rbrakk>
+   \<Longrightarrow> frgt \<turnstile> (IF t1\<noteq>0 THEN t2 ELSE t3,bs,xs) \<Rightarrow>\<^bsup>T\<^esup> l2" |
 hIfFalse:
-  "\<lbrakk>reg \<turnstile> (t1,bs,xs) \<Rightarrow>\<^bsup>T1\<^esup> Value v1; v1 = 0; reg \<turnstile> (t3,bs,xs) \<Rightarrow>\<^bsup>T3\<^esup> l3; T = T1@T3\<rbrakk>
-   \<Longrightarrow> reg \<turnstile> (IF t1\<noteq>0 THEN t2 ELSE t3,bs,xs) \<Rightarrow>\<^bsup>T\<^esup> l3" |
+  "\<lbrakk>frgt \<turnstile> (t1,bs,xs) \<Rightarrow>\<^bsup>T1\<^esup> Value v1; v1 = 0; frgt \<turnstile> (t3,bs,xs) \<Rightarrow>\<^bsup>T3\<^esup> l3; T = T1@T3\<rbrakk>
+   \<Longrightarrow> frgt \<turnstile> (IF t1\<noteq>0 THEN t2 ELSE t3,bs,xs) \<Rightarrow>\<^bsup>T\<^esup> l3" |
 hCall:
-  "\<lbrakk>(g, T_g) = reg gr; length vs = length ts; length Ts = length ts;
-    \<forall>i < length ts. reg \<turnstile> (ts ! i,bs,xs) \<Rightarrow>\<^bsup>Ts ! i\<^esup> Value (vs ! i);
+  "\<lbrakk>(g, T_g) = frgt gr; length vs = length ts; length Ts = length ts;
+    \<forall>i < length ts. frgt \<turnstile> (ts ! i,bs,xs) \<Rightarrow>\<^bsup>Ts ! i\<^esup> Value (vs ! i);
     T = concat Ts @ [(gr,vs)]; v = g vs\<rbrakk>
-   \<Longrightarrow> reg \<turnstile> (hCall gr ts,bs,xs) \<Rightarrow>\<^bsup>T\<^esup> Value v" |
+   \<Longrightarrow> frgt \<turnstile> (hCall gr ts,bs,xs) \<Rightarrow>\<^bsup>T\<^esup> Value v" |
 hTail:
   "\<lbrakk>length vs = length ts; length Ts = length ts;
-    \<forall>i < length ts. reg \<turnstile> (ts ! i,bs,xs) \<Rightarrow>\<^bsup>Ts ! i\<^esup> Value (vs ! i);
+    \<forall>i < length ts. frgt \<turnstile> (ts ! i,bs,xs) \<Rightarrow>\<^bsup>Ts ! i\<^esup> Value (vs ! i);
     T = concat Ts\<rbrakk>
-   \<Longrightarrow> reg \<turnstile> (hTAIL ts,bs,xs) \<Rightarrow>\<^bsup>T\<^esup> Tail vs"
+   \<Longrightarrow> frgt \<turnstile> (hTAIL ts,bs,xs) \<Rightarrow>\<^bsup>T\<^esup> Tail vs"
 
 lemmas htrace_to_leaf_induct = htrace_to_leaf.induct[split_format(complete)]
 
@@ -214,95 +205,95 @@ We show: if there is a semantics, either:
 *)
 
 lemma trace_val_to_semantics0:
-  assumes "reg \<turnstile> (t,bs,xs) \<Rightarrow>\<^bsup>(T :: trace)\<^esup> l" "l = Value v"
-  shows "(f,reg) \<turnstile> (t,bs,xs) \<Rightarrow>\<^bsup> interp_trace reg T \<^esup> v"
+  assumes "frgt \<turnstile> (t,bs,xs) \<Rightarrow>\<^bsup>(T :: trace)\<^esup> l" "l = Value v"
+  shows "(f,frgt) \<turnstile> (t,bs,xs) \<Rightarrow>\<^bsup> interp_trace frgt T \<^esup> v"
 using assms proof (induction arbitrary: v rule: htrace_to_leaf_induct)
-  case (hCall g T_g reg gr vs ts Ts bs xs T v)
-  let ?zs = "map (interp_trace reg) Ts"
+  case (hCall g T_g frgt gr vs ts Ts bs xs T v)
+  let ?zs = "map (interp_trace frgt) Ts"
   show ?case
   proof
-    have "interp_trace reg [(gr,vs)] = T_g vs"
-      unfolding interp_trace_def interp_trace_item_def using hCall split_from_reg by simp
-    then show "interp_trace reg T = sum_list ?zs + T_g vs"
+    have "interp_trace frgt [(gr,vs)] = T_g vs"
+      unfolding interp_trace_def interp_trace_item_def using hCall split_from_frgt by simp
+    then show "interp_trace frgt T = sum_list ?zs + T_g vs"
       using hCall interp_trace_concat_is_sum_map interp_trace_append by simp
   next
     show "g vs = v" using hCall by simp
   qed (simp_all add: hCall)
-qed (simp_all add: interp_trace_def hbig_step_t.intros)
+qed (auto simp add: interp_trace_def hbig_step_t.intros)
 
 theorem trace_val_to_semantics:
-  assumes "reg \<turnstile> (t,bs,xs) \<Rightarrow>\<^bsup>T\<^esup> Value v"
-  shows "(f,reg) \<turnstile> (t,bs,xs) \<Rightarrow>\<^bsup> interp_trace reg T \<^esup> v"
+  assumes "frgt \<turnstile> (t,bs,xs) \<Rightarrow>\<^bsup>T\<^esup> Value v"
+  shows "(f,frgt) \<turnstile> (t,bs,xs) \<Rightarrow>\<^bsup> interp_trace frgt T \<^esup> v"
   using assms trace_val_to_semantics0 by blast
 
 
 lemma trace_tail_to_semantics0:
-  assumes "reg \<turnstile> (t,bs,xs) \<Rightarrow>\<^bsup>(T :: trace)\<^esup> l" "l = Tail xs'"
+  assumes "frgt \<turnstile> (t,bs,xs) \<Rightarrow>\<^bsup>(T :: trace)\<^esup> l" "l = Tail xs'"
   assumes "invar t"
-  assumes "(f,reg) \<turnstile> (f,[],xs') \<Rightarrow>\<^bsup>z\<^esup> v"
-  shows "(f,reg) \<turnstile> (t,bs,xs) \<Rightarrow>\<^bsup> interp_trace reg T + z + 1 \<^esup> v"
+  assumes "(f,frgt) \<turnstile> (f,[],xs') \<Rightarrow>\<^bsup>z\<^esup> v"
+  shows "(f,frgt) \<turnstile> (t,bs,xs) \<Rightarrow>\<^bsup> interp_trace frgt T + z + 1 \<^esup> v"
   (* TODO: could probably get this proof a bit shorter/cleaner, OK for now *)
 using assms proof (induction arbitrary: rule: htrace_to_leaf_induct)
-  case (hLet reg t1 bs xs T1 v1 t2 T2 l2 T)
+  case (hLet frgt t1 bs xs T1 v1 t2 T2 l2 T)
   show ?case
   proof
-    show "interp_trace reg T + z + 1 = (interp_trace reg T1) + (interp_trace reg T2 + z + 1)"
+    show "interp_trace frgt T + z + 1 = (interp_trace frgt T1) + (interp_trace frgt T2 + z + 1)"
       using hLet interp_trace_append by simp
   next
-    show "(f, reg) \<turnstile> (t1, bs, xs) \<Rightarrow>\<^bsup>interp_trace reg T1\<^esup> v1"
+    show "(f, frgt) \<turnstile> (t1, bs, xs) \<Rightarrow>\<^bsup>interp_trace frgt T1\<^esup> v1"
       using hLet trace_val_to_semantics by simp
   next
-    show "(f, reg) \<turnstile> (t2, v1 # bs, xs) \<Rightarrow>\<^bsup>interp_trace reg T2 + z + 1\<^esup>  v"
+    show "(f, frgt) \<turnstile> (t2, v1 # bs, xs) \<Rightarrow>\<^bsup>interp_trace frgt T2 + z + 1\<^esup>  v"
       using hLet by simp
   qed
 next
-  case (hIfTrue reg t1 bs xs T1 v1 t2 T2 l2 T t3)
+  case (hIfTrue frgt t1 bs xs T1 v1 t2 T2 l2 T t3)
   show ?case
   proof (rule hbig_step_t.hIfTrue)
-    show "(f, reg) \<turnstile> (t1, bs, xs) \<Rightarrow>\<^bsup>interp_trace reg T1\<^esup> v1"
+    show "(f, frgt) \<turnstile> (t1, bs, xs) \<Rightarrow>\<^bsup>interp_trace frgt T1\<^esup> v1"
       using hIfTrue trace_val_to_semantics by simp
   next
     show "v1 \<noteq> 0" using hIfTrue by simp
   next
-    show "(f, reg) \<turnstile> (t2, bs, xs) \<Rightarrow>\<^bsup>interp_trace reg T2 + z + 1\<^esup> v" using hIfTrue by simp
+    show "(f, frgt) \<turnstile> (t2, bs, xs) \<Rightarrow>\<^bsup>interp_trace frgt T2 + z + 1\<^esup> v" using hIfTrue by simp
   next
-    show "interp_trace reg T + z + 1 = (interp_trace reg T1) + (interp_trace reg T2 + z + 1)"
+    show "interp_trace frgt T + z + 1 = (interp_trace frgt T1) + (interp_trace frgt T2 + z + 1)"
       using hIfTrue by simp
   qed
 next
-  case (hIfFalse reg t1 bs xs T1 v1 t3 T3 l3 T t2)
+  case (hIfFalse frgt t1 bs xs T1 v1 t3 T3 l3 T t2)
   show ?case
   proof (rule hbig_step_t.hIfFalse)
-    show "(f, reg) \<turnstile> (t1, bs, xs) \<Rightarrow>\<^bsup>interp_trace reg T1\<^esup> v1"
+    show "(f, frgt) \<turnstile> (t1, bs, xs) \<Rightarrow>\<^bsup>interp_trace frgt T1\<^esup> v1"
       using hIfFalse trace_val_to_semantics by simp
   next
     show "v1 = 0" using hIfFalse by simp
   next
-    show "(f, reg) \<turnstile> (t3, bs, xs) \<Rightarrow>\<^bsup>interp_trace reg T3 + z + 1\<^esup> v" using hIfFalse by simp
+    show "(f, frgt) \<turnstile> (t3, bs, xs) \<Rightarrow>\<^bsup>interp_trace frgt T3 + z + 1\<^esup> v" using hIfFalse by simp
   next
-    show "interp_trace reg T + z + 1 = (interp_trace reg T1) + (interp_trace reg T3 + z + 1)"
+    show "interp_trace frgt T + z + 1 = (interp_trace frgt T1) + (interp_trace frgt T3 + z + 1)"
       using hIfFalse by simp
   qed
 next
-  case (hTail vs ts Ts reg bs xs T)
-  let ?zs = "map (interp_trace reg) Ts"
+  case (hTail vs ts Ts frgt bs xs T)
+  let ?zs = "map (interp_trace frgt) Ts"
   show ?case
   proof
-    show "interp_trace reg T + z + 1 = sum_list ?zs + z + 1"
+    show "interp_trace frgt T + z + 1 = sum_list ?zs + z + 1"
       using hTail interp_trace_concat_is_sum_map interp_trace_append by simp
-  next show "\<forall>i<length ts. (f, reg) \<turnstile> (ts ! i, bs, xs) \<Rightarrow>\<^bsup>?zs ! i\<^esup> vs ! i"
+  next show "\<forall>i<length ts. (f, frgt) \<turnstile> (ts ! i, bs, xs) \<Rightarrow>\<^bsup>?zs ! i\<^esup> vs ! i"
       using hTail[simplified] nth_map trace_val_to_semantics by simp
   next show "length vs = length ts" using hTail by simp
-  next show "(f, reg) \<turnstile> (f, [], vs) \<Rightarrow>\<^bsup>z\<^esup> v" using hTail by simp
-  next show "length (map (interp_trace reg) Ts) = length ts" using hTail by simp
+  next show "(f, frgt) \<turnstile> (f, [], vs) \<Rightarrow>\<^bsup>z\<^esup> v" using hTail by simp
+  next show "length (map (interp_trace frgt) Ts) = length ts" using hTail by simp
   qed
 qed simp_all
 
 theorem trace_tail_to_semantics:
   assumes "invar t"
-  assumes "reg \<turnstile> (t,bs,xs) \<Rightarrow>\<^bsup>T\<^esup> Tail xs'"
-  assumes "(f,reg) \<turnstile> (f,[],xs') \<Rightarrow>\<^bsup>z\<^esup> v"
-  shows "(f,reg) \<turnstile> (t,bs,xs) \<Rightarrow>\<^bsup> interp_trace reg T + z + 1 \<^esup> v"
+  assumes "frgt \<turnstile> (t,bs,xs) \<Rightarrow>\<^bsup>T\<^esup> Tail xs'"
+  assumes "(f,frgt) \<turnstile> (f,[],xs') \<Rightarrow>\<^bsup>z\<^esup> v"
+  shows "(f,frgt) \<turnstile> (t,bs,xs) \<Rightarrow>\<^bsup> interp_trace frgt T + z + 1 \<^esup> v"
   using assms trace_tail_to_semantics0 by blast
 
 
@@ -311,8 +302,8 @@ theorem trace_tail_to_semantics:
 
 lemma sem_to_trace_non_tailE:
   assumes "\<not> tails t"
-  assumes "(f,reg) \<turnstile> (t,bs,xs) \<Rightarrow>\<^bsup> z \<^esup> v"
-  obtains T :: trace where "reg \<turnstile> (t,bs,xs) \<Rightarrow>\<^bsup>T\<^esup> Value v" "interp_trace reg T = z"
+  assumes "(f,frgt) \<turnstile> (t,bs,xs) \<Rightarrow>\<^bsup> z \<^esup> v"
+  obtains T :: trace where "frgt \<turnstile> (t,bs,xs) \<Rightarrow>\<^bsup>T\<^esup> Value v" "interp_trace frgt T = z"
   using assms(2,1) apply (induction rule: hbig_step_t_induct)
   apply (metis HOL_TCN_Timing.tails.simps(2) htrace_to_leaf.hLet interp_trace_append)
   apply (metis htrace_to_leaf.hLetBound interp_trace_def list.map(1) sum_list.Nil)
@@ -320,7 +311,7 @@ lemma sem_to_trace_non_tailE:
   apply (metis htrace_to_leaf.hNumber interp_trace_def list.map(1) sum_list.Nil)
   apply (metis HOL_TCN_Timing.tails.simps(3) htrace_to_leaf.hIfTrue interp_trace_append)
   apply (metis HOL_TCN_Timing.tails.simps(3) htrace_to_leaf.hIfFalse interp_trace_append)
-  sorry (* TODO *)
+  oops (* TODO *)
 
 lemma sem_to_trace_inductionI:
   assumes "P' \<or> (\<exists>xs'. Q1' xs' \<and> Q2' xs')"
@@ -330,153 +321,155 @@ lemma sem_to_trace_inductionI:
   shows "\<exists>T. P T \<or> (\<exists>xs'. Q1 T xs' \<and> Q2 T xs')"
   using assms by blast
 
+(* oops
 lemma sem_to_traceE:
   assumes "invar t"
-  assumes "(f,reg) \<turnstile> (t,bs,xs) \<Rightarrow>\<^bsup>z\<^esup> v"
+  assumes "(f,frgt) \<turnstile> (t,bs,xs) \<Rightarrow>\<^bsup>z\<^esup> v"
   shows "\<exists>T.
-    (reg \<turnstile> (t,bs,xs) \<Rightarrow>\<^bsup>T\<^esup> Value v) \<or>
-    (\<exists>xs'. reg \<turnstile> (t,bs,xs) \<Rightarrow>\<^bsup>T\<^esup> Tail xs'
-           \<and> (f,reg) \<turnstile> (f,[],xs') \<Rightarrow>\<^bsup>z - interp_trace reg T - 1\<^esup> v)"
+    (frgt \<turnstile> (t,bs,xs) \<Rightarrow>\<^bsup>T\<^esup> Value v) \<or>
+    (\<exists>xs'. frgt \<turnstile> (t,bs,xs) \<Rightarrow>\<^bsup>T\<^esup> Tail xs'
+           \<and> (f,frgt) \<turnstile> (f,[],xs') \<Rightarrow>\<^bsup>z - interp_trace frgt T - 1\<^esup> v)"
 using assms(2,1) proof (induction rule: hbig_step_t_induct)
-  case (hLet f reg t1 bs xs z1 v1 t2 z2 v z)
+  case (hLet f frgt t1 bs xs z1 v1 t2 z2 v z)
 
   from sem_to_trace_non_tailE hLet.hyps(1) obtain T1 where
-    T1: "reg \<turnstile> (t1,bs,xs) \<Rightarrow>\<^bsup>T1\<^esup> Value v1" "interp_trace reg T1 = z1"
+    T1: "frgt \<turnstile> (t1,bs,xs) \<Rightarrow>\<^bsup>T1\<^esup> Value v1" "interp_trace frgt T1 = z1"
     using hLet.prems invar.simps by blast
   from hLet.IH(2) obtain T2 where
-      "(reg \<turnstile> (t2,v1#bs,xs) \<Rightarrow>\<^bsup>T2\<^esup> Value v) \<or>
-       (\<exists>xs'. reg \<turnstile> (t2,v1#bs,xs) \<Rightarrow>\<^bsup>T2\<^esup> Tail xs' \<and>
-              (f, reg) \<turnstile> (f,[],xs') \<Rightarrow>\<^bsup>z2 - interp_trace reg T2 - 1\<^esup> v)"
+      "(frgt \<turnstile> (t2,v1#bs,xs) \<Rightarrow>\<^bsup>T2\<^esup> Value v) \<or>
+       (\<exists>xs'. frgt \<turnstile> (t2,v1#bs,xs) \<Rightarrow>\<^bsup>T2\<^esup> Tail xs' \<and>
+              (f, frgt) \<turnstile> (f,[],xs') \<Rightarrow>\<^bsup>z2 - interp_trace frgt T2 - 1\<^esup> v)"
     using hLet.prems by auto
   then show ?case proof (rule sem_to_trace_inductionI)
-    assume "reg \<turnstile> (t2,v1#bs,xs) \<Rightarrow>\<^bsup>T2\<^esup> Value v"
-    then show "reg \<turnstile> (LET t1 IN t2,bs,xs) \<Rightarrow>\<^bsup>T1@T2\<^esup> Value v"
+    assume "frgt \<turnstile> (t2,v1#bs,xs) \<Rightarrow>\<^bsup>T2\<^esup> Value v"
+    then show "frgt \<turnstile> (LET t1 IN t2,bs,xs) \<Rightarrow>\<^bsup>T1@T2\<^esup> Value v"
       using T1 htrace_to_leaf.intros by simp
   next
     fix xs'
-    assume "reg \<turnstile> (t2, v1 # bs, xs) \<Rightarrow>\<^bsup>T2\<^esup>  Tail xs'"
-    then show "reg \<turnstile> (LET t1 IN t2, bs, xs) \<Rightarrow>\<^bsup>T1@T2\<^esup>  Tail xs'"
+    assume "frgt \<turnstile> (t2, v1 # bs, xs) \<Rightarrow>\<^bsup>T2\<^esup>  Tail xs'"
+    then show "frgt \<turnstile> (LET t1 IN t2, bs, xs) \<Rightarrow>\<^bsup>T1@T2\<^esup>  Tail xs'"
       using T1 htrace_to_leaf.intros by simp
   next
     fix xs'
-    assume "(f, reg) \<turnstile> (f, [], xs') \<Rightarrow>\<^bsup>z2 - interp_trace reg T2 - 1\<^esup>  v"
-    then show "(f, reg) \<turnstile> (f, [], xs') \<Rightarrow>\<^bsup>z - interp_trace reg (T1 @ T2) - 1\<^esup>  v"
+    assume "(f, frgt) \<turnstile> (f, [], xs') \<Rightarrow>\<^bsup>z2 - interp_trace frgt T2 - 1\<^esup>  v"
+    then show "(f, frgt) \<turnstile> (f, [], xs') \<Rightarrow>\<^bsup>z - interp_trace frgt (T1 @ T2) - 1\<^esup>  v"
       using hLet T1 htrace_to_leaf.intros interp_trace_append by simp
   qed
 next
-  case (hLetBound v bs n a b xs)
-  then have "b \<turnstile> (hLetBound n, bs, xs) \<Rightarrow>\<^bsup> [] \<^esup> Value v" using htrace_to_leaf.intros by simp
+  case (hLetBound n bs a b xs)
+  then have "b \<turnstile> (hLetBound n, bs, xs) \<Rightarrow>\<^bsup> [] \<^esup> Value (bs ! n)" using htrace_to_leaf.intros by simp
   then show ?case by blast
 next
-  case (hArg v xs n a b bs)
-  then have "b \<turnstile> (hArg n, bs, xs) \<Rightarrow>\<^bsup> [] \<^esup> Value v" using htrace_to_leaf.intros by simp
+  case (hArg n xs a b bs)
+  then have "b \<turnstile> (hArg n, bs, xs) \<Rightarrow>\<^bsup> [] \<^esup> Value (xs ! n)" using htrace_to_leaf.intros by simp
   then show ?case by blast
 next
   case (hNumber a b n bs xs)
   then have "b \<turnstile> (hNumber n, bs, xs) \<Rightarrow>\<^bsup> [] \<^esup> Value n" using htrace_to_leaf.intros by simp
   then show ?case by blast
 next
-  case (hIfTrue f reg t1 bs xs z1 v1 t2 z2 v2 z t3)
+  case (hIfTrue f frgt t1 bs xs z1 v1 t2 z2 v2 z t3)
   from sem_to_trace_non_tailE hIfTrue.hyps(1) obtain T1 where
-    T1: "reg \<turnstile> (t1,bs,xs) \<Rightarrow>\<^bsup>T1\<^esup> Value v1" "interp_trace reg T1 = z1"
+    T1: "frgt \<turnstile> (t1,bs,xs) \<Rightarrow>\<^bsup>T1\<^esup> Value v1" "interp_trace frgt T1 = z1"
     using hIfTrue.prems invar.simps by blast
   from hIfTrue.IH(2) obtain T2 where
-      "(reg \<turnstile> (t2,bs,xs) \<Rightarrow>\<^bsup>T2\<^esup> Value v2) \<or>
-       (\<exists>xs'. reg \<turnstile> (t2,bs,xs) \<Rightarrow>\<^bsup>T2\<^esup> Tail xs' \<and>
-              (f, reg) \<turnstile> (f,[],xs') \<Rightarrow>\<^bsup>z2 - interp_trace reg T2 - 1\<^esup> v2)"
+      "(frgt \<turnstile> (t2,bs,xs) \<Rightarrow>\<^bsup>T2\<^esup> Value v2) \<or>
+       (\<exists>xs'. frgt \<turnstile> (t2,bs,xs) \<Rightarrow>\<^bsup>T2\<^esup> Tail xs' \<and>
+              (f, frgt) \<turnstile> (f,[],xs') \<Rightarrow>\<^bsup>z2 - interp_trace frgt T2 - 1\<^esup> v2)"
     using hIfTrue.prems by auto
   then show ?case proof (rule sem_to_trace_inductionI)
-    assume "reg \<turnstile> (t2,bs,xs) \<Rightarrow>\<^bsup>T2\<^esup> Value v2"
-    then show "reg \<turnstile> (IF t1\<noteq>0 THEN t2 ELSE t3,bs,xs) \<Rightarrow>\<^bsup>T1@T2\<^esup> Value v2"
+    assume "frgt \<turnstile> (t2,bs,xs) \<Rightarrow>\<^bsup>T2\<^esup> Value v2"
+    then show "frgt \<turnstile> (IF t1\<noteq>0 THEN t2 ELSE t3,bs,xs) \<Rightarrow>\<^bsup>T1@T2\<^esup> Value v2"
       using hIfTrue T1 htrace_to_leaf.intros by simp
   next
     fix xs'
-    assume "reg \<turnstile> (t2,bs,xs) \<Rightarrow>\<^bsup>T2\<^esup> Tail xs'"
-    then show "reg \<turnstile> (IF t1\<noteq>0 THEN t2 ELSE t3,bs,xs) \<Rightarrow>\<^bsup>T1@T2\<^esup> Tail xs'"
+    assume "frgt \<turnstile> (t2,bs,xs) \<Rightarrow>\<^bsup>T2\<^esup> Tail xs'"
+    then show "frgt \<turnstile> (IF t1\<noteq>0 THEN t2 ELSE t3,bs,xs) \<Rightarrow>\<^bsup>T1@T2\<^esup> Tail xs'"
       using hIfTrue T1 htrace_to_leaf.intros by simp
   next
     fix xs'
-    assume "(f,reg) \<turnstile> (f,[],xs') \<Rightarrow>\<^bsup>z2 - interp_trace reg T2 - 1\<^esup>  v2"
-    then show "(f,reg) \<turnstile> (f,[],xs') \<Rightarrow>\<^bsup>z - interp_trace reg (T1@T2) - 1\<^esup> v2"
+    assume "(f,frgt) \<turnstile> (f,[],xs') \<Rightarrow>\<^bsup>z2 - interp_trace frgt T2 - 1\<^esup>  v2"
+    then show "(f,frgt) \<turnstile> (f,[],xs') \<Rightarrow>\<^bsup>z - interp_trace frgt (T1@T2) - 1\<^esup> v2"
       using hIfTrue T1 htrace_to_leaf.intros interp_trace_append by simp
   qed
 next
-  case (hIfFalse f reg t1 bs xs z1 v1 t3 z2 v2 z t2)
+  case (hIfFalse f frgt t1 bs xs z1 v1 t3 z2 v2 z t2)
   from sem_to_trace_non_tailE hIfFalse.hyps(1) obtain T1 where
-    T1: "reg \<turnstile> (t1,bs,xs) \<Rightarrow>\<^bsup>T1\<^esup> Value v1" "interp_trace reg T1 = z1"
+    T1: "frgt \<turnstile> (t1,bs,xs) \<Rightarrow>\<^bsup>T1\<^esup> Value v1" "interp_trace frgt T1 = z1"
     using hIfFalse.prems invar.simps by blast
   from hIfFalse.IH(2) obtain T2 where
-      "(reg \<turnstile> (t3,bs,xs) \<Rightarrow>\<^bsup>T2\<^esup> Value v2) \<or>
-       (\<exists>xs'. reg \<turnstile> (t3,bs,xs) \<Rightarrow>\<^bsup>T2\<^esup> Tail xs' \<and>
-              (f,reg) \<turnstile> (f,[],xs') \<Rightarrow>\<^bsup>z2 - interp_trace reg T2 - 1\<^esup> v2)"
+      "(frgt \<turnstile> (t3,bs,xs) \<Rightarrow>\<^bsup>T2\<^esup> Value v2) \<or>
+       (\<exists>xs'. frgt \<turnstile> (t3,bs,xs) \<Rightarrow>\<^bsup>T2\<^esup> Tail xs' \<and>
+              (f,frgt) \<turnstile> (f,[],xs') \<Rightarrow>\<^bsup>z2 - interp_trace frgt T2 - 1\<^esup> v2)"
     using hIfFalse.prems by auto
   then show ?case proof (rule sem_to_trace_inductionI)
-    assume "reg \<turnstile> (t3,bs,xs) \<Rightarrow>\<^bsup>T2\<^esup> Value v2"
-    then show "reg \<turnstile> (IF t1\<noteq>0 THEN t2 ELSE t3,bs,xs) \<Rightarrow>\<^bsup>T1@T2\<^esup> Value v2"
+    assume "frgt \<turnstile> (t3,bs,xs) \<Rightarrow>\<^bsup>T2\<^esup> Value v2"
+    then show "frgt \<turnstile> (IF t1\<noteq>0 THEN t2 ELSE t3,bs,xs) \<Rightarrow>\<^bsup>T1@T2\<^esup> Value v2"
       using hIfFalse T1 htrace_to_leaf.intros by simp
   next
     fix xs'
-    assume "reg \<turnstile> (t3,bs,xs) \<Rightarrow>\<^bsup>T2\<^esup> Tail xs'"
-    then show "reg \<turnstile> (IF t1\<noteq>0 THEN t2 ELSE t3,bs,xs) \<Rightarrow>\<^bsup>T1@T2\<^esup> Tail xs'"
+    assume "frgt \<turnstile> (t3,bs,xs) \<Rightarrow>\<^bsup>T2\<^esup> Tail xs'"
+    then show "frgt \<turnstile> (IF t1\<noteq>0 THEN t2 ELSE t3,bs,xs) \<Rightarrow>\<^bsup>T1@T2\<^esup> Tail xs'"
       using hIfFalse T1 htrace_to_leaf.intros by simp
   next
     fix xs'
-    assume "(f,reg) \<turnstile> (f,[],xs') \<Rightarrow>\<^bsup>z2 - interp_trace reg T2 - 1\<^esup>  v2"
-    then show "(f,reg) \<turnstile> (f,[],xs') \<Rightarrow>\<^bsup>z - interp_trace reg (T1@T2) - 1\<^esup> v2"
+    assume "(f,frgt) \<turnstile> (f,[],xs') \<Rightarrow>\<^bsup>z2 - interp_trace frgt T2 - 1\<^esup>  v2"
+    then show "(f,frgt) \<turnstile> (f,[],xs') \<Rightarrow>\<^bsup>z - interp_trace frgt (T1@T2) - 1\<^esup> v2"
       using hIfFalse T1 htrace_to_leaf.intros interp_trace_append by simp
   qed
 next
-  case (hCall g T_g reg gr zs ts vs f bs xs v' z')
+  case (hCall g T_g frgt gr zs ts vs f bs xs v' z')
   then show ?case sorry (* TODO *)
 next
-  case (hTAIL zs ts vs f reg bs xs z' v' z'')
+  case (hTAIL zs ts vs f frgt bs xs z' v' z'')
   then show ?case sorry
 qed
 
 (* TODO is this better *)
 lemma sem_to_traceE':
   assumes "invar t"
-  assumes "(f,reg) \<turnstile> (t,bs,xs) \<Rightarrow>\<^bsup>z\<^esup> v"
+  assumes "(f,frgt) \<turnstile> (t,bs,xs) \<Rightarrow>\<^bsup>z\<^esup> v"
   obtains T where "
-    (reg \<turnstile> (t,bs,xs) \<Rightarrow>\<^bsup>T\<^esup> Value v) \<or>
-    (\<exists>xs'. reg \<turnstile> (t,bs,xs) \<Rightarrow>\<^bsup>T\<^esup> Tail xs'
-           \<and> (f,reg) \<turnstile> (f,[],xs') \<Rightarrow>\<^bsup>z - interp_trace reg T - 1\<^esup> v)"
-  using assms sem_to_traceE by blast
+    (frgt \<turnstile> (t,bs,xs) \<Rightarrow>\<^bsup>T\<^esup> Value v) \<or>
+    (\<exists>xs'. frgt \<turnstile> (t,bs,xs) \<Rightarrow>\<^bsup>T\<^esup> Tail xs'
+           \<and> (f,frgt) \<turnstile> (f,[],xs') \<Rightarrow>\<^bsup>z - interp_trace frgt T - 1\<^esup> v)"
+  using assms sem_to_traceE by blast *)
 
 lemma sem_to_trace_existsE:
   assumes "invar t"
-  assumes "(f,reg) \<turnstile> (t,bs,xs) \<Rightarrow>\<^bsup> z \<^esup> v"
-  obtains T :: trace and l where "reg \<turnstile> (t,bs,xs) \<Rightarrow>\<^bsup>T\<^esup> l"
-  using sem_to_traceE assms by blast
+  assumes "(f,frgt) \<turnstile> (t,bs,xs) \<Rightarrow>\<^bsup> z \<^esup> v"
+  obtains T :: trace and l where "frgt \<turnstile> (t,bs,xs) \<Rightarrow>\<^bsup>T\<^esup> l"
+  (* using sem_to_traceE assms by blast *)
+  oops
 
 (*
 lemma trace_val_from_semantics:
   assumes "invar t" (* ? *)
-  assumes "(f,reg) \<turnstile> (t,bs,xs) \<Rightarrow>\<^bsup> z \<^esup> v1"
-  assumes "reg \<turnstile> (t,bs,xs) \<Rightarrow>\<^bsup>T\<^esup> Value v2"
-  shows "v1 = v2 \<and> interp_trace reg T = z"
+  assumes "(f,frgt) \<turnstile> (t,bs,xs) \<Rightarrow>\<^bsup> z \<^esup> v1"
+  assumes "frgt \<turnstile> (t,bs,xs) \<Rightarrow>\<^bsup>T\<^esup> Value v2"
+  shows "v1 = v2 \<and> interp_trace frgt T = z"
   sorry
 
 lemma non_tails_trace: (* useful/meaningful? *)
   assumes "\<not> tails t"
-  assumes "(f,reg) \<turnstile> (t,bs,xs) \<Rightarrow>\<^bsup> z \<^esup> v"
-  obtains T where "reg \<turnstile> (t,bs,xs) \<Rightarrow>\<^bsup> T \<^esup> Value v" "interp_trace reg T = z"
+  assumes "(f,frgt) \<turnstile> (t,bs,xs) \<Rightarrow>\<^bsup> z \<^esup> v"
+  obtains T where "frgt \<turnstile> (t,bs,xs) \<Rightarrow>\<^bsup> T \<^esup> Value v" "interp_trace frgt T = z"
   using trace_exists_non_tail trace_val_from_semantics assms no_tails_invar by blast
 
 lemma trace_tail_from_semantics:
   assumes "invar t" (* ? *)
-  assumes "(f,reg) \<turnstile> (t,bs,xs) \<Rightarrow>\<^bsup> z \<^esup> v"
-  assumes "reg \<turnstile> (t,bs,xs) \<Rightarrow>\<^bsup>T\<^esup> Tail xs'"
-  shows "(f,reg) \<turnstile> (f,[],xs') \<Rightarrow>\<^bsup>z - interp_trace reg T - 1\<^esup> v"
+  assumes "(f,frgt) \<turnstile> (t,bs,xs) \<Rightarrow>\<^bsup> z \<^esup> v"
+  assumes "frgt \<turnstile> (t,bs,xs) \<Rightarrow>\<^bsup>T\<^esup> Tail xs'"
+  shows "(f,frgt) \<turnstile> (f,[],xs') \<Rightarrow>\<^bsup>z - interp_trace frgt T - 1\<^esup> v"
   sorry
 
 lemma trace_from_semantics:
   assumes "invar t"
-  assumes "(f,reg) \<turnstile> (t,bs,xs) \<Rightarrow>\<^bsup> z \<^esup> v1"
-  assumes "reg \<turnstile> (t,bs,xs) \<Rightarrow>\<^bsup> T :: trace \<^esup> l"
+  assumes "(f,frgt) \<turnstile> (t,bs,xs) \<Rightarrow>\<^bsup> z \<^esup> v1"
+  assumes "frgt \<turnstile> (t,bs,xs) \<Rightarrow>\<^bsup> T :: trace \<^esup> l"
   shows "(case l of
       Value v2 \<Rightarrow> v2 = v1
-    | Tail xs' \<Rightarrow> (f,reg) \<turnstile> (f,[],xs') \<Rightarrow>\<^bsup>z - interp_trace reg T - 1\<^esup> v)"
+    | Tail xs' \<Rightarrow> (f,frgt) \<turnstile> (f,[],xs') \<Rightarrow>\<^bsup>z - interp_trace frgt T - 1\<^esup> v)"
   using trace_val_from_semantics[OF assms(1) assms(2)] trace_tail_from_semantics assms sorry
 
 *)
