IMP/HOL_TCN_To_IMP.thy
@@ -1,38 +1,112 @@
 theory HOL_TCN_To_IMP
   (* TODO: move file *)
   imports IMP_Tailcall_Traces HOL_TCN_Timing Fresh
-(* "HOL-Library.Log_Nat"  *)
 begin
+
+(* function name \<Rightarrow> (argument registers' names \<times> IMP command \<times> return register's name *)
+type_synonym com_registry = "fun_ref \<Rightarrow> (vname list \<times> com \<times> vname)"
+abbreviation "args_from_crgt (crgt :: com_registry) name \<equiv> fst (crgt name)"
+abbreviation "com_from_crgt (crgt :: com_registry) name \<equiv> fst (snd (crgt name))"
+abbreviation "ret_from_crgt (crgt :: com_registry) name \<equiv> snd (snd (crgt name))"
+(* TODO: use these abbrev. *)
+
+definition "null = (\<lambda>_. undefined)"
+
+
+(* fresh *)
 
 (* let us switch between definitions easily *)
 abbreviation "fresh' \<equiv> Fresh.fresh"
 
+(* TODO: this should go in Fresh (but then can't swap out fresh' anymore) *)
+definition "make_nth_fresh stale name = fresh' stale o ((@) name) o string_of_nat" 
+definition "make_n_fresh stale name n = map (make_nth_fresh stale name) [0..<n]"
+
+lemma inj_make_nth_fresh[simp]: "inj (make_nth_fresh stale name)"
+  by (simp add: inj_append2 inj_compose inj_fresh inj_string_of_nat make_nth_fresh_def)
+
+lemma distinct_make_n_fresh[simp]: "distinct (make_n_fresh stale name n)"
+  unfolding make_n_fresh_def using distinct_map inj_make_nth_fresh distinct_upt inj_on_subset by blast
+
+lemma make_n_fresh_not_in_stale: "set (make_n_fresh stale name n) \<inter> set stale = {}"
+  unfolding make_n_fresh_def make_nth_fresh_def using fresh_not_in_stale by auto
+
+value "make_n_fresh [''f.args.2.0'', ''f.args.2.1'', ''f.args.3.0''] ''f.args.'' 5"
+
+
+lemma inj_inj_on: fixes A assumes "inj f" shows "inj_on f A" using assms inj_on_subset by auto
+(* lemma inj_neq: fixes A assumes "inj_on f A" "x \<noteq> y" "x \<in> A" "y \<in> A" shows "f x \<noteq> f y" using assms  *)
+  (* thm inj_on_contraD[where A = UNIV, simplified] *)
+lemma none_equal_not_in: fixes A shows "(\<forall>y\<in>A. x \<noteq> y) \<longleftrightarrow> x \<notin> A" by blast
+lemma some_equal_in: fixes A shows "(\<exists>y\<in>A. x = y) \<longleftrightarrow> x \<in> A" by blast
+
 (*
-definition map_fresh where
-  "map_fresh stale name f xs =
-    snd ((foldl (\<lambda>(st0, xs') x. (fresh' st0 name # st0, xs' @ [f st0 (fresh' st0 name) x])) (stale, [])) xs)"
+find_theorems "_ \<notin> _" "inj_on"
 
-value "map_fresh [] ''x'' (\<lambda>v vs (x :: nat). (x, v, vs)) [1, 2, 3]"
+lemma fixes A assumes "inj_on f (insert x A)" "x \<notin> A" shows "f x \<notin> f ` A" using assms by blast *)
 
-definition "fresh_n (n :: nat) stale name = snd (fold (\<lambda>_ (st0, r).
-  let x = fresh' st0 name in (x # st0, r @ [(x, st0)])) [1..int n] (stale, []))" *)
 
-(* definition "make_n (n :: nat) name = [name @ string_of_nat i . i <- [0..<n]]" *)
-definition "make_n_fresh n stale name = map (fresh' stale o ((@) name) o string_of_nat) [0..<n]"
+(* t_seqs *)
 
-lemma distinct_make_n_fresh: "distinct (make_n_fresh n stale name)"
-unfolding make_n_fresh_def proof (subst distinct_map, standard)
-  show "inj_on (fresh' stale \<circ> (@) name \<circ> string_of_nat) (set [0..<n])"
-    using comp_inj_on inj_string_of_nat inj_append2 Fresh.inj_fresh inj_on_subset[where A = UNIV, simplified]
-    by metis
-qed simp
+lemma tbig_step_t_tSeq_assoc:
+  (* from Compile_HOL_Nat_To_IMP *)
+  shows "C \<turnstile> (c1 ;; (c2 ;; c3), s) \<Rightarrow>\<^bsup>t\<^esup> s' \<longleftrightarrow> C \<turnstile> (c1 ;; c2 ;; c3, s) \<Rightarrow>\<^bsup>t\<^esup> s'"
+  by auto
 
-value "make_n_fresh 5 [''f.args.2.0'', ''f.args.2.1'', ''f.args.3.0''] ''f.args.''"
+lemma tbig_step_t_tSeq_Skip_id1[simp]: "f \<turnstile> (tSKIP;; c, s) \<Rightarrow>\<^bsup>Suc z\<^esup> t \<longleftrightarrow> f \<turnstile> (c, s) \<Rightarrow>\<^bsup>z\<^esup> t"
+  by fastforce
 
-(* definition "foldr1 f xs = foldr f (butlast xs) (last xs)" *)
-(* definition "t_seqs ts = foldr1 tSeq ts" (* (if ts = [] then tSKIP else  *) *)
-definition "t_seqs ts = foldr tSeq ts" (* (if ts = [] then tSKIP else  *)
+lemma tbig_step_t_tSeq_Skip_id2[simp]: "f \<turnstile> (c;; tSKIP, s) \<Rightarrow>\<^bsup>Suc z\<^esup> t \<longleftrightarrow> f \<turnstile> (c, s) \<Rightarrow>\<^bsup>z\<^esup> t"
+  by fastforce
+
+definition "t_seqs ts = foldr tSeq ts"
+abbreviation "t_seqs' ts \<equiv> t_seqs ts tSKIP"
 value "t_seqs ([c1, c2, c3]) c4"
+
+lemma t_seqs_nil[simp]: "t_seqs [] c = c" unfolding t_seqs_def by simp
+lemma t_seqs_cons[simp]: "t_seqs (c1 # cs) c = c1;; t_seqs cs c" unfolding t_seqs_def by simp
+
+lemma t_seqs_append[simp]: "t_seqs (cs1 @ cs2) c = t_seqs cs1 (t_seqs cs2 c)"
+  by (induction cs1) auto
+
+lemmas t_seqs_rewrite = t_seqs_nil t_seqs_cons t_seqs_append
+
+lemma t_seqs_Seq: "f \<turnstile> (t_seqs cs (c1;; c2),s) \<Rightarrow>\<^bsup>z\<^esup> t \<longleftrightarrow> f \<turnstile> (t_seqs cs c1;; c2,s) \<Rightarrow>\<^bsup>z\<^esup> t"
+  by (induction cs arbitrary: s z) fastforce+
+
+lemma t_seqs'_snoc: "f \<turnstile> (t_seqs' (cs @ [c]),s) \<Rightarrow>\<^bsup>Suc z\<^esup> t \<longleftrightarrow> f \<turnstile> (t_seqs cs c,s) \<Rightarrow>\<^bsup>z\<^esup> t"
+  using t_seqs_Seq by simp
+
+lemma t_seqs'_t_seqs:
+  shows "f \<turnstile> (t_seqs' cs;; c,s) \<Rightarrow>\<^bsup>Suc z\<^esup> t \<longleftrightarrow> f \<turnstile> (t_seqs cs c,s) \<Rightarrow>\<^bsup>z\<^esup> t"
+proof
+  assume "f \<turnstile> (t_seqs cs c, s) \<Rightarrow>\<^bsup>z\<^esup> t" then show "f \<turnstile> (t_seqs' cs;; c, s) \<Rightarrow>\<^bsup>Suc z\<^esup> t"
+    by (induction cs arbitrary: s z) fastforce+
+next
+  assume "f \<turnstile> (t_seqs' cs;; c, s) \<Rightarrow>\<^bsup>Suc z\<^esup> t"
+  then show "f \<turnstile> (t_seqs cs c, s) \<Rightarrow>\<^bsup>z\<^esup> t"
+  proof (induction cs arbitrary: s z)
+    case Nil then show ?case by auto
+  next
+    case (Cons c1 cs)
+    then have "f \<turnstile> (c1;; (t_seqs' cs;; c), s) \<Rightarrow>\<^bsup>Suc z\<^esup>  t" using tbig_step_t_tSeq_assoc by simp
+    then obtain z1 s2 z2 where "f \<turnstile> (c1, s) \<Rightarrow>\<^bsup>z1\<^esup> s2" "f \<turnstile> (t_seqs' cs;; c, s2) \<Rightarrow>\<^bsup>Suc z2\<^esup> t" "Suc z = z1 + Suc z2"
+      using bigstep_progressE tSeq_tE by metis
+    then show ?case using Cons.IH by auto
+  qed
+qed
+
+lemma t_seqs'_append: "f \<turnstile> (t_seqs' cs1;; t_seqs' cs2,s) \<Rightarrow>\<^bsup>Suc z\<^esup> t \<longleftrightarrow> f \<turnstile> (t_seqs' (cs1 @ cs2),s) \<Rightarrow>\<^bsup>z\<^esup> t"
+  using t_seqs'_t_seqs by simp
+
+lemma t_seqs_append_t_seqs': "f \<turnstile> (t_seqs' cs1;; t_seqs' cs2;; c,s) \<Rightarrow>\<^bsup>Suc (Suc z)\<^esup> t \<longleftrightarrow> f \<turnstile> (t_seqs (cs1 @ cs2) c,s) \<Rightarrow>\<^bsup>z\<^esup> t"
+  apply (induction cs1)
+  apply (simp add: t_seqs'_t_seqs tbig_step_t_tSeq_assoc[symmetric])
+  apply (simp add: t_seqs'_append)
+  apply (metis t_seqs'_t_seqs t_seqs_cons)
+  done
+
+lemmas tbig_step_t_t_seqs_rewrite = t_seqs_Seq t_seqs'_snoc t_seqs'_t_seqs t_seqs'_append t_seqs_append_t_seqs'
 
 (* lemma foldr1_append: assumes "xs \<noteq> []" "ys \<noteq> []" shows "foldr1 f (xs @ ys) = foldr tSeq xs (foldr1 tSeq ys)" *)
 
@@ -51,23 +125,38 @@ lemma non_tails_tseqs[simp]:
   (* apply simp sledgehammer *)
    (* apply (induction xs) unfolding t_seqs_def foldr1_def apply simp_all *)
 
-abbreviation "mapi f xs \<equiv> snd (fold (\<lambda>x (i, ys). (i + 1, ys @ [f i x])) xs (0, []))"
+abbreviation "mapi' n ys f xs \<equiv> snd (fold (\<lambda>x (i, ys). (i + 1, ys @ [f i x])) xs (n, ys))"
+abbreviation "mapi \<equiv> mapi' 0 []"
 
-lemma mapi_map2[simp]: "mapi f xs = map2 f [0..<length xs] xs"
-proof-
-  have gen: "snd (fold (\<lambda>x (i, ys). (i + 1, ys @ [f i x])) xs (length ys, ys))
-             = ys @ map2 f [length ys..<length ys + length xs] xs" for xs ys
-  proof (induction xs arbitrary: ys)
-    case (Cons x xs)
-    have "[length ys..<length ys + length (x # xs)]
-          = length ys # [Suc (length ys)..<length ys + length (x # xs)]"
-      using upt_conv_Cons upt_rec by simp
-    thus ?case using Cons[of "ys @ [f (length ys) x]"] by simp
-  qed simp
-  from gen[where ys = "[]"] show "mapi f xs = map2 f [0..<length xs] xs" by simp
-qed
+lemma mapi'_map:
+  "mapi' (length ys) ys f xs = ys @ map (\<lambda>i. f i (xs ! (i - length ys))) [length ys..<length ys + length xs]"
+proof (induction xs arbitrary: ys)
+  case (Cons x xs)
+  let ?y = "f (length ys) x"
+  have "ys @ map (\<lambda>i. f i ((x # xs) ! (i - length ys))) [length ys..<length ys + length (x # xs)] =
+      ys @ ?y # map (\<lambda>i. f i ((x # xs) ! (i - length ys))) [Suc (length ys) ..< length ys + length (x # xs)]"
+    using upt_rec by simp
+  also have "... = ys @ ?y # map (\<lambda>i. f i (xs ! (i - Suc (length ys)))) [Suc (length ys)..<length ys + length (x # xs)]"
+    by (simp add: nth_Cons')
+  also have "... = mapi' (length ys) ys f (x # xs)" using Cons[where ys = "ys @ [?y]"] by simp
+  finally show ?case by fastforce
+qed simp
 
-find_theorems "?t \<in> set (map ?f ?xs)"
+corollary mapi_map: "mapi f xs = map (\<lambda>i. f i (xs ! i)) [0..<length xs]"
+  using mapi'_map[where ys = "[]" and f = f and xs = xs] by simp
+
+lemma mapi'_map2: "mapi' (length ys) ys f xs = ys @ map2 f [length ys..<length ys + length xs] xs"
+proof (induction xs arbitrary: ys)
+  case (Cons x xs)
+  have "[length ys..<length ys + length (x # xs)]
+        = length ys # [Suc (length ys)..<length ys + length (x # xs)]"
+    using upt_conv_Cons upt_rec by simp
+  thus ?case using Cons[of "ys @ [f (length ys) x]"] by simp
+qed simp
+
+corollary mapi_map2: "mapi f xs = map2 f [0..<length xs] xs"
+  using mapi'_map2[where ys = "[]" and f = f and xs = xs] by simp
+
 
 lemma map_obtain: assumes "y \<in> set (map f xs)" obtains x where "y = f x" "x \<in> set xs" using assms by auto
 
@@ -84,58 +173,70 @@ qed
 
 
 fun to_imp_tc ::
-    "vname list \<Rightarrow> thol_ctxt
+    "vname list \<Rightarrow> com_registry
     \<Rightarrow> vname list \<Rightarrow> vname \<Rightarrow> vname list \<Rightarrow> thol
     \<Rightarrow> tcom" where
   (* f_args: list of argument registers' names
-     ctxt: see type def
+     crgt: see type def
      bs: names of bound variables
      r: return register name
      stale: variable names that must not be written to *)
   (* fresh variables: need two conditions:
     - must not overwrite live variables
     - must not be overwritten before any use *)
-  "to_imp_tc f_args ctxt bs r stale (hIf t1 t2 t3) =
+  "to_imp_tc f_args crgt bs r stale (hIf t1 t2 t3) =
     (let x_var = fresh' stale ''If.x'';
-         c1 = to_imp_tc f_args ctxt bs x_var stale t1;
-         c2 = to_imp_tc f_args ctxt bs r stale t2;
-         c3 = to_imp_tc f_args ctxt bs r stale t3
+         c1 = to_imp_tc f_args crgt bs x_var stale t1;
+         c2 = to_imp_tc f_args crgt bs r stale t2;
+         c3 = to_imp_tc f_args crgt bs r stale t3
       in tSeq c1 (tIf x_var c2 c3))" |
-  "to_imp_tc f_args ctxt bs r stale (hLet t1 t2) =
+  "to_imp_tc f_args crgt bs r stale (hLet t1 t2) =
     (let x_var = fresh' stale ''Let.x'';
-         c1 = to_imp_tc f_args ctxt bs x_var stale t1;
-         c2 = to_imp_tc f_args ctxt (x_var # bs) r (x_var # stale) t2
+         c1 = to_imp_tc f_args crgt bs x_var stale t1;
+         c2 = to_imp_tc f_args crgt (x_var # bs) r (x_var # stale) t2
       in tSeq c1 c2)" |
-  "to_imp_tc f_args ctxt bs r stale (hLetBound n) = tAssign r (A (V (bs ! n)))" |
-  "to_imp_tc f_args ctxt bs r stale (hArg n) = tAssign r (A (V (f_args ! n)))" |
-  "to_imp_tc f_args ctxt bs r stale (hNumber n) = tAssign r (A (N n))" |
+  "to_imp_tc f_args crgt bs r stale (hLetBound n) = tAssign r (A (V (bs ! n)))" |
+  "to_imp_tc f_args crgt bs r stale (hArg n) = tAssign r (A (V (f_args ! n)))" |
+  "to_imp_tc f_args crgt bs r stale (hNumber n) = tAssign r (A (N n))" |
   (* TODO: call/TAIL cases could be written more nicely, but need termination proofs.
       On the other hand, this more closely follows the written presentation. *)
   (* could use nth consistently *)
-  "to_imp_tc f_args ctxt bs r stale (hCall g ts) =
-    (let (g_args, c_g, g_ret) = ctxt g;
+  "to_imp_tc f_args crgt bs r stale (hCall g ts) =
+    (let (g_args, c_g, g_ret) = crgt g;
+         xs = make_n_fresh stale ''Call.x.'' (length ts);
+         cs1 = mapi (\<lambda>i t. to_imp_tc f_args crgt bs (xs ! i) (xs @ stale) t) ts;
+         cs2 = map (\<lambda>i. tAssign (g_args ! i) (A (V (xs ! i)))) [0..<length ts]
+      in t_seqs (cs1 @ cs2) (tSeq (tCall c_g g_ret) (tAssign r (A (V g_ret)))))" |
+  "to_imp_tc f_args crgt bs r stale (hTAIL ts) =
+    (let xs = make_n_fresh stale ''TAIL.x.'' (length ts);
+         cs1 = mapi (\<lambda>i t. to_imp_tc f_args crgt bs (xs ! i) (xs @ stale) t) ts;
+         cs2 = map (\<lambda>i. tAssign (f_args ! i) (A (V (xs ! i)))) [0..<length ts]
+      in t_seqs (cs1 @ cs2) tTAIL)"
+(*
+  "to_imp_tc f_args crgt bs r stale (hCall g ts) =
+    (let (g_args, c_g, g_ret) = crgt g;
          xs = make_n_fresh (length ts) stale ''Call.x.'';
-         cs1 = mapi (\<lambda>i t. to_imp_tc f_args ctxt bs (xs ! i) (xs @ stale) t) ts;
+         cs1 = mapi (\<lambda>i t. to_imp_tc f_args crgt bs (xs ! i) (xs @ stale) t) ts;
          cs2 = mapi (\<lambda>i t. tAssign (g_args ! i) (A (V (xs ! i)))) ts
       in t_seqs (cs1 @ cs2) (tSeq (tCall c_g g_ret) (tAssign r (A (V g_ret)))))" |
-  "to_imp_tc f_args ctxt bs r stale (hTAIL ts) =
+  "to_imp_tc f_args crgt bs r stale (hTAIL ts) =
     (let xs = make_n_fresh (length ts) stale ''TAIL.x.'';
-         cs1 = mapi (\<lambda>i t. to_imp_tc f_args ctxt bs (xs ! i) (xs @ stale) t) ts;
+         cs1 = mapi (\<lambda>i t. to_imp_tc f_args crgt bs (xs ! i) (xs @ stale) t) ts;
          cs2 = mapi (\<lambda>i t. tAssign (f_args ! i) (A (V (xs ! i)))) ts
-      in t_seqs (cs1 @ cs2) tTAIL)"
+      in t_seqs (cs1 @ cs2) tTAIL)" *)
 
-lemma to_imp_nontail: "\<not> HOL_TCN_Timing.tails t \<Longrightarrow> \<not> IMP_Tailcall.tails (to_imp_tc f_args ctxt bs r stale t)"
+lemma to_imp_nontail: "\<not> HOL_TCN_Timing.tails t \<Longrightarrow> \<not> IMP_Tailcall.tails (to_imp_tc f_args crgt bs r stale t)"
 proof (induction t arbitrary: bs r stale)
   case (hCall g ts)
-  let ?xs = "make_n_fresh (length ts) stale ''Call.x.''"
-  let ?cs1 = "mapi (\<lambda>i t. to_imp_tc f_args ctxt bs (?xs ! i) (?xs @ stale) t) ts"
-  let ?cs2 = "mapi (\<lambda>i t. tAssign (args_from_ctxt ctxt g ! i) (A (V (?xs ! i)))) ts"
+  let ?xs = "make_n_fresh stale ''Call.x.'' (length ts)"
+  let ?cs1 = "mapi (\<lambda>i t. to_imp_tc f_args crgt bs (?xs ! i) (?xs @ stale) t) ts"
+  let ?cs2 = "mapi (\<lambda>i t. tAssign (args_from_crgt crgt g ! i) (A (V (?xs ! i)))) ts"
 
   have 1: "\<forall>s \<in> set ?cs1. \<not> IMP_Tailcall.tails s"
   proof
     fix s
     assume 1: "s \<in> set ?cs1"
-    obtain i t where "s = to_imp_tc f_args ctxt bs (?xs ! i) (?xs @ stale) t" "t \<in> set ts"
+    obtain i t where "s = to_imp_tc f_args crgt bs (?xs ! i) (?xs @ stale) t" "t \<in> set ts"
       using mapi_obtain[OF 1] by blast
     with hCall show "\<not> IMP_Tailcall.tails s" by simp
   qed
@@ -150,18 +251,18 @@ proof (induction t arbitrary: bs r stale)
     done
 qed (simp_all add: Let_def) (* why do all the other cases go through by simp ???? TODO: figure it out and clean up these proofs *)
 
-lemma to_imp_invar: "HOL_TCN_Timing.invar t \<Longrightarrow> IMP_Tailcall.invar (to_imp_tc f_args ctxt bs r stale t)"
+lemma to_imp_invar: "HOL_TCN_Timing.invar t \<Longrightarrow> IMP_Tailcall.invar (to_imp_tc f_args crgt bs r stale t)"
 proof (induction t arbitrary: bs r stale)
   case (hCall g ts)
-  let ?xs = "make_n_fresh (length ts) stale ''Call.x.''"
-  let ?cs1 = "mapi (\<lambda>i t. to_imp_tc f_args ctxt bs (?xs ! i) (?xs @ stale) t) ts"
-  let ?cs2 = "mapi (\<lambda>i t. tAssign (fst (ctxt g) ! i) (A (V (?xs ! i)))) ts"
+  let ?xs = "make_n_fresh stale ''Call.x.'' (length ts)"
+  let ?cs1 = "mapi (\<lambda>i t. to_imp_tc f_args crgt bs (?xs ! i) (?xs @ stale) t) ts"
+  let ?cs2 = "mapi (\<lambda>i t. tAssign (fst (crgt g) ! i) (A (V (?xs ! i)))) ts"
 
   have 1: "\<forall>s \<in> set ?cs1. \<not> IMP_Tailcall.tails s"
   proof
     fix s
     assume 1: "s \<in> set ?cs1"
-    obtain i t where "s = to_imp_tc f_args ctxt bs (?xs ! i) (?xs @ stale) t" "t \<in> set ts"
+    obtain i t where "s = to_imp_tc f_args crgt bs (?xs ! i) (?xs @ stale) t" "t \<in> set ts"
       using mapi_obtain[OF 1] by blast
     with hCall to_imp_nontail show "\<not> IMP_Tailcall.tails s" by simp
   qed
@@ -175,15 +276,15 @@ proof (induction t arbitrary: bs r stale)
     done
 next
   case (hTAIL ts)
-  let ?xs = "make_n_fresh (length ts) stale ''TAIL.x.''"
-  let ?cs1 = "mapi (\<lambda>i t. to_imp_tc f_args ctxt bs (?xs ! i) (?xs @ stale) t) ts"
+  let ?xs = "make_n_fresh stale ''TAIL.x.'' (length ts)"
+  let ?cs1 = "mapi (\<lambda>i t. to_imp_tc f_args crgt bs (?xs ! i) (?xs @ stale) t) ts"
   let ?cs2 = "mapi (\<lambda>i t. tAssign (f_args ! i) (A (V (?xs ! i)))) ts"
 
   have 1: "\<forall>s \<in> set ?cs1. \<not> IMP_Tailcall.tails s"
   proof
     fix s
     assume 1: "s \<in> set ?cs1"
-    obtain i t where "s = to_imp_tc f_args ctxt bs (?xs ! i) (?xs @ stale) t" "t \<in> set ts"
+    obtain i t where "s = to_imp_tc f_args crgt bs (?xs ! i) (?xs @ stale) t" "t \<in> set ts"
       using mapi_obtain[OF 1] by blast
     with hTAIL to_imp_nontail show "\<not> IMP_Tailcall.tails s" by simp
   qed
@@ -198,12 +299,12 @@ next
 qed (simp_all add: Let_def to_imp_nontail)
 
 
-definition "reserved_regs f_args ctxt bs t =
-    (f_args @ bs @ concat (map (fst o ctxt) (calls t)) @ map (snd o snd o ctxt) (calls t))"
+definition "reserved_regs f_args crgt bs t =
+    (f_args @ bs @ concat (map (args_from_crgt crgt o fst) (calls t)) @ map (ret_from_crgt crgt o fst) (calls t))"
 
 (* mark argument/return registers of all called functions and of f itself as stale *)
-definition "to_imp_tc' f_args ctxt bs r t =
-  to_imp_tc f_args ctxt bs r (reserved_regs f_args ctxt bs t) t"
+definition "to_imp_tc' f_args crgt bs r t =
+  to_imp_tc f_args crgt bs r (reserved_regs f_args crgt bs t) t"
 (* TODO: right-assoc ? *)
 
 definition "h_let_1 = hLet (hNumber 7) (hLetBound 0)"
